good progress

HOL_To_IMP/Refinements/HOL_TCN_To_IMP_Temp.thy
@@ -22,7 +22,11 @@ lemma disjoint_subset2:
   shows "A \<inter>\<^sub>\<emptyset> B"
   using assms by blast
 
-definition "compiler_args_invar crgt f_args bs keep t \<longleftrightarrow>
+lemma fresh_not_in_stale_subset: assumes "set stale' \<subseteq> set stale" shows "fresh stale name \<notin> set stale'"
+  using fresh_not_in_stale assms by blast
+
+
+definition "compiler_invar crgt f_args bs keep t \<longleftrightarrow>
   HOL_TCN_Timing.invar t
   \<and> distinct f_args
   \<and> set f_args \<inter>\<^sub>\<emptyset> set (call_registers crgt t)
@@ -30,8 +34,8 @@ definition "compiler_args_invar crgt f_args bs keep t \<longleftrightarrow>
   \<and> set bs \<inter>\<^sub>\<emptyset> set f_args
   \<and> set keep \<inter>\<^sub>\<emptyset> set f_args
   \<and> set keep \<inter>\<^sub>\<emptyset> set (call_registers crgt t)
-  \<and> (\<forall>g\<in>fst ` set (calls t). distinct (args_from_crgt crgt g))
-  \<and> (\<forall>(g,ts)\<in>set (calls t). length ts = length (args_from_crgt crgt g))"
+  \<and> (\<forall>g\<in>set (calls' t). distinct (args_from_crgt crgt g))
+  \<and> (\<forall>(g,n)\<in>set (calls_n t). n = length (args_from_crgt crgt g))"
 (*
 - The term must be tail-recursive, i.e. satisfy the invariant.
 
@@ -65,16 +69,159 @@ definition "compiler_args_invar crgt f_args bs keep t \<longleftrightarrow>
   We special-case the keep/r conflict: instead of requiring keep and r to be disjoint, the
   correctness theorems show that "keep" except "r" is preserved.
 
-- At each call site, the correct number of arguments must be provided to the called function.
+- At each (TODO: tail: len ... = len f_args, needs new function to collect tail calls) call site, the correct number of arguments must be provided to the called function.
+
+Note that this is not the *weakest* possible invariant, but that would
+significantly complicate the invariant with no obvious benefit.
 *)
 
-lemma compiler_args_invar_subset:
-  assumes "invar t"
-  assumes "set (calls t) \<subseteq> set (calls t')"
-  assumes "compiler_args_invar crgt f_args bs keep t'"
-  shows "compiler_args_invar crgt f_args bs keep t"
-  using disjoint_subset2[where B = "set (call_registers crgt t)" and B' = "set (call_registers crgt t')"]
-  using assms call_registers_set unfolding compiler_args_invar_def split_beta by auto
+lemma compiler_invarE[elim]:
+  assumes "compiler_invar crgt f_args bs keep t"
+  shows
+    "HOL_TCN_Timing.invar t"
+    "distinct f_args"
+    "set f_args \<inter>\<^sub>\<emptyset> set (call_registers crgt t)"
+    "set bs \<inter>\<^sub>\<emptyset> set (call_registers crgt t)"
+    "set bs \<inter>\<^sub>\<emptyset> set f_args"
+    "set keep \<inter>\<^sub>\<emptyset> set f_args"
+    "set keep \<inter>\<^sub>\<emptyset> set (call_registers crgt t)"
+    "\<And>g. g \<in> set (calls' t) \<Longrightarrow> distinct (args_from_crgt crgt g)" (* what's the canonical way to write this? *)
+    "\<And>g n. (g,n)\<in>set (calls_n t) \<Longrightarrow> n = length (args_from_crgt crgt g)"
+  using assms unfolding compiler_invar_def by auto
+
+lemma compiler_invarI[intro]:
+  assumes
+    "HOL_TCN_Timing.invar t"
+    "distinct f_args"
+    "set f_args \<inter>\<^sub>\<emptyset> set (call_registers crgt t)"
+    "set bs \<inter>\<^sub>\<emptyset> set (call_registers crgt t)"
+    "set bs \<inter>\<^sub>\<emptyset> set f_args"
+    "set keep \<inter>\<^sub>\<emptyset> set f_args"
+    "set keep \<inter>\<^sub>\<emptyset> set (call_registers crgt t)"
+    "\<And>g. g \<in> set (calls' t) \<Longrightarrow> distinct (args_from_crgt crgt g)"
+    "\<And>g n. (g,n)\<in>set (calls_n t) \<Longrightarrow> n = length (args_from_crgt crgt g)"
+  shows "compiler_invar crgt f_args bs keep t"
+  using assms unfolding compiler_invar_def by blast
+
+lemma compiler_invar_subset:
+  assumes invar: "invar t"
+  assumes calls: "set (calls t) \<subseteq> set (calls t')" (* subset on calls_n would be enough... *)
+  assumes comp_invar: "compiler_invar crgt f_args bs keep t'"
+  shows "compiler_invar crgt f_args bs keep t"
+proof
+  have "set (call_registers crgt t) \<subseteq> set (call_registers crgt t')"
+    using calls calls'_set unfolding call_registers_def by auto
+  then show
+      "set f_args \<inter>\<^sub>\<emptyset> set (call_registers crgt t)"
+      "set bs \<inter>\<^sub>\<emptyset> set (call_registers crgt t)"
+      "set keep \<inter>\<^sub>\<emptyset> set (call_registers crgt t)"
+    using compiler_invarE[OF comp_invar] by blast+
+next
+  fix g assume "g \<in> set (calls' t)"
+  then have "g \<in> set (calls' t')" using calls calls'_set by auto
+  then show "distinct (args_from_crgt crgt g)" using comp_invar by auto
+next
+  fix g n assume "(g,n) \<in> set (calls_n t)"
+  then have "(g,n) \<in> set (calls_n t')" using calls calls_n_set by auto
+  then show "n = length (args_from_crgt crgt g)" using comp_invar by auto
+qed (auto simp add: invar compiler_invarE[OF comp_invar])
+
+lemma compiler_invar_let:
+  fixes crgt f_args bs keep t1 t2
+  assumes comp_invar: "compiler_invar crgt f_args bs keep (LET t1 IN t2)"
+  defines "r \<equiv> fresh' (stale_registers f_args crgt bs keep LET t1 IN t2) ''Let.x''"
+  shows
+    "compiler_invar crgt f_args bs keep t1"
+    "compiler_invar crgt f_args (r # bs) (r # keep) t2"
+proof -
+  have "invar t1" using comp_invar unfolding compiler_invar_def by simp
+  then show "compiler_invar crgt f_args bs keep t1"
+    using comp_invar compiler_invar_subset[where t' = "LET t1 IN t2"] by simp
+next
+  have "invar t2" using comp_invar unfolding compiler_invar_def by simp
+  then have "compiler_invar crgt f_args bs keep t2"
+    using comp_invar compiler_invar_subset[where t' = "LET t1 IN t2"] by simp
+
+  moreover have "r \<notin> set f_args"
+    unfolding r_def stale_registers_def
+    using fresh_not_in_stale set_append by fastforce
+  moreover have "r \<notin> set (call_registers crgt t2)"
+  unfolding r_def proof (rule fresh_not_in_stale_subset)
+    show "set (call_registers crgt t2) \<subseteq> set (stale_registers f_args crgt bs keep LET t1 IN t2)"
+      unfolding stale_registers_def call_registers_def using calls'_set by auto
+  qed
+
+  ultimately show "compiler_invar crgt f_args (r # bs) (r # keep) t2"
+    unfolding compiler_invar_def by auto
+qed
+
+lemma compiler_invar_if:
+  assumes "compiler_invar crgt f_args bs keep (IF t1\<noteq>0 THEN t2 ELSE t3)"
+  shows
+    "compiler_invar crgt f_args bs keep t1"
+    "compiler_invar crgt f_args bs keep t2"
+    "compiler_invar crgt f_args bs keep t3"
+proof -
+  have "HOL_TCN_Timing.invar t1" using assms unfolding compiler_invar_def by simp
+  moreover have "set (calls t1) \<subseteq> set (calls (IF t1\<noteq>0 THEN t2 ELSE t3))" by fastforce
+  ultimately show "compiler_invar crgt f_args bs keep t1"
+    using assms compiler_invar_subset by metis
+next
+  have "HOL_TCN_Timing.invar t2" using assms unfolding compiler_invar_def by simp
+  moreover have "set (calls t2) \<subseteq> set (calls (IF t1\<noteq>0 THEN t2 ELSE t3))" by fastforce
+  ultimately show "compiler_invar crgt f_args bs keep t2"
+    using assms compiler_invar_subset by metis
+next
+  have "HOL_TCN_Timing.invar t3" using assms unfolding compiler_invar_def by simp
+  moreover have "set (calls t3) \<subseteq> set (calls (IF t1\<noteq>0 THEN t2 ELSE t3))" by fastforce
+  ultimately show "compiler_invar crgt f_args bs keep t3"
+    using assms compiler_invar_subset by metis
+qed
+
+lemma compiler_invar_call:
+  fixes f_args crgt bs keep gr ts
+  assumes compiler_invar: "compiler_invar crgt f_args bs keep (hCall gr ts)"
+  defines "xs \<equiv> make_n_fresh (stale_registers f_args crgt bs keep (hCall gr ts)) ''Call.x.'' (length ts)"
+  assumes t: "t \<in> set ts"
+  shows "compiler_invar crgt f_args bs (xs @ keep) t"
+proof -
+  have "HOL_TCN_Timing.invar t" using compiler_invar t unfolding compiler_invar_def by simp
+  with t compiler_invar compiler_invar_subset[where t = t and t' = "hCall gr ts"]
+  have inv: "compiler_invar crgt f_args bs keep t" by fastforce
+
+  show "compiler_invar crgt f_args bs (xs @ keep) t"
+  proof
+    have "set (call_registers crgt t) \<subseteq> set (call_registers crgt (hCall gr ts))"
+      using t calls'_set unfolding call_registers_def by auto
+    then have "set xs \<inter>\<^sub>\<emptyset> set f_args" "set xs \<inter>\<^sub>\<emptyset> set (call_registers crgt t)"
+      unfolding xs_def stale_registers_def using make_n_fresh_not_in_stale by fastforce+
+    then show "set (xs @ keep) \<inter>\<^sub>\<emptyset> set f_args" "set (xs @ keep) \<inter>\<^sub>\<emptyset> set (call_registers crgt t)"
+      using inv unfolding compiler_invar_def by fastforce+
+  qed (simp_all add: compiler_invarE[OF inv])
+qed
+
+lemma compiler_invar_tail:
+  fixes f_args crgt bs keep gr ts
+  assumes compiler_invar: "compiler_invar crgt f_args bs keep (hTAIL ts)"
+  defines "xs \<equiv> make_n_fresh (stale_registers f_args crgt bs keep (hTAIL ts)) ''TAIL.x.'' (length ts)"
+  assumes t: "t \<in> set ts"
+  shows "compiler_invar crgt f_args bs (xs @ keep) t"
+proof -
+  have "HOL_TCN_Timing.invar t" using compiler_invar t unfolding compiler_invar_def by simp
+  with t compiler_invar compiler_invar_subset[where t = t and t' = "hTAIL ts"]
+  have inv: "compiler_invar crgt f_args bs keep t" by fastforce
+
+  show "compiler_invar crgt f_args bs (xs @ keep) t"
+  proof
+    have "set (call_registers crgt t) \<subseteq> set (call_registers crgt (hTAIL ts))"
+      using t calls'_set unfolding call_registers_def by auto
+    then have "set xs \<inter>\<^sub>\<emptyset> set f_args" "set xs \<inter>\<^sub>\<emptyset> set (call_registers crgt t)"
+      unfolding xs_def stale_registers_def using make_n_fresh_not_in_stale by fastforce+
+    then show "set (xs @ keep) \<inter>\<^sub>\<emptyset> set f_args" "set (xs @ keep) \<inter>\<^sub>\<emptyset> set (call_registers crgt t)"
+      using inv unfolding compiler_invar_def by fastforce+
+  qed (simp_all add: compiler_invarE[OF inv])
+qed
+
 
 (* the "state" of the HOL-TCN execution (args, bounds) is related
    to the state of the IMP-TC execution *)
@@ -92,6 +239,49 @@ definition "relate_rgt_correctness frgt crgt fs \<longleftrightarrow> (\<forall>
   \<forall>s. terminates_with_res_IMP (com_from_crgt crgt f) s (ret_from_crgt crgt f) (f_from_frgt frgt f (lookup_args crgt f s)))"
 
 
+definition rel_trace_call :: "com_registry \<Rightarrow> fun_ref \<Rightarrow> nat list \<Rightarrow> com \<Rightarrow> state \<Rightarrow> bool" where
+  "rel_trace_call crgt gr gargs gcom gs \<longleftrightarrow> com_from_crgt crgt gr = gcom \<and> lookup_args crgt gr gs = gargs"
+definition rel_trace_calls :: "com_registry \<Rightarrow> HOL_TCN_Timing.trace \<Rightarrow> IMP_Tailcall_Traces.call_trace \<Rightarrow> bool" where
+  "rel_trace_calls crgt hT cT \<longleftrightarrow>
+    length hT = length cT \<and>
+    list_all (\<lambda>((gr,gargs),(gcom,gs)). rel_trace_call crgt gr gargs gcom gs) (zip hT cT)"
+(* "rel_trace_calls crgt hT cT \<longleftrightarrow>
+    length hT = length cT \<and>
+    (\<forall>i < length hT. let (gr, gargs) = hT ! i; (gcom, gs) = cT ! i in
+                     rel_trace_call crgt gr gargs gcom gs)" *)
+fun rel_leaf_state :: "com_registry \<Rightarrow> vname list \<Rightarrow> vname \<Rightarrow> leaf_state \<Rightarrow> state \<Rightarrow> bool \<Rightarrow> bool" where
+  "rel_leaf_state crgt _      r (Value v) s l \<longleftrightarrow> \<not> l \<and> s       r        = v " |
+  "rel_leaf_state crgt f_args _ (Tail vs) s l \<longleftrightarrow>   l \<and> lookups f_args s = vs"
+
+definition rel_trace_to_leaf ::
+    "com_registry \<Rightarrow> vname list \<Rightarrow> vname \<Rightarrow>
+      HOL_TCN_Timing.trace \<Rightarrow> leaf_state \<Rightarrow>
+        IMP_Tailcall_Traces.call_trace \<Rightarrow> state \<Rightarrow> bool \<Rightarrow> bool" where
+  "rel_trace_to_leaf crgt f_args r hT hl cT s cl \<longleftrightarrow>
+    rel_trace_calls crgt hT cT \<and> rel_leaf_state crgt f_args r hl s cl"
+
+(* lemma
+  assumes "length xs = length ys"
+  shows "(\<forall>i<length xs. P (xs ! i) (ys ! i)) = list_all (\<lambda>(x, y). P x y) (zip xs ys)"
+   apply (induction rule: snoc_list_induct2[OF assms])  *)
+
+lemma rel_trace_to_leaf_cl:
+  shows "rel_trace_to_leaf crgt f_args r hT (Value v) cT s cl \<Longrightarrow> \<not> cl"
+    and "rel_trace_to_leaf crgt f_args r hT (Tail vs) cT s cl \<Longrightarrow> cl"
+  unfolding rel_trace_to_leaf_def by simp_all
+
+lemma rel_trace_calls_append:
+  assumes "rel_trace_calls crgt hT1 cT1"
+  assumes "rel_trace_calls crgt hT2 cT2"
+  shows "rel_trace_calls crgt (hT1 @ hT2) (cT1 @ cT2)" using assms unfolding rel_trace_calls_def by simp
+
+lemma rel_trace_to_leaf_append:
+  assumes "rel_trace_calls crgt hT1 cT1"
+  assumes "rel_trace_to_leaf crgt f_args r hT2 hl cT2 s cl"
+  shows "rel_trace_to_leaf crgt f_args r (hT1 @ hT2) hl (cT1 @ cT2) s cl"
+  using assms unfolding rel_trace_to_leaf_def rel_trace_calls_def by auto
+
+
 lemma snoc_obtain:
   assumes "xs \<noteq> []"
   obtains x xs' where "xs = xs' @ [x]"
@@ -102,7 +292,7 @@ lemma snoc_list_induct2 [case_names len Nil snoc]:
   assumes nil: "P [] []"
   assumes snoc: "\<And>xs x ys y. length xs = length ys \<Longrightarrow> P xs ys \<Longrightarrow> P (xs @ [x]) (ys @ [y])"
   shows "P xs ys"
-proof-
+proof -
   let ?P = "\<lambda>xs ys. P (rev xs) (rev ys)"
   have "length (rev xs) = length (rev ys)" using len by simp
   then have "?P (rev xs) (rev ys)"
@@ -116,7 +306,7 @@ lemma snoc_list_induct3 [case_names len1 len2 Nil snoc]:
   assumes nil: "P [] [] []"
   assumes snoc: "\<And>xs x ys y zs z. length xs = length ys \<Longrightarrow> length ys = length zs \<Longrightarrow> P xs ys zs \<Longrightarrow> P (xs @ [x]) (ys @ [y]) (zs @ [z])"
   shows "P xs ys zs"
-proof-
+proof -
   let ?P = "\<lambda>xs ys zs. P (rev xs) (rev ys) (rev zs)"
   have "length (rev xs) = length (rev ys)" "length (rev ys) = length (rev zs)" using len by simp_all
   then have "?P (rev xs) (rev ys) (rev zs)"
@@ -125,13 +315,33 @@ proof-
   then show "P xs ys zs" by simp
 qed
 
+lemma snoc_list_induct4 [case_names len1 len2 len3 Nil snoc]:
+  assumes len: "length xs1 = length xs2" "length xs2 = length xs3" "length xs3 = length xs4"
+  assumes nil: "P [] [] [] []"
+  assumes snoc: "\<And>xs1 x1 xs2 x2 xs3 x3 xs4 x4.
+    length xs1 = length xs2 \<Longrightarrow> length xs2 = length xs3 \<Longrightarrow> length xs3 = length xs4 \<Longrightarrow>
+    P xs1 xs2 xs3 xs4 \<Longrightarrow> P (xs1 @ [x1]) (xs2 @ [x2]) (xs3 @ [x3]) (xs4 @ [x4])"
+  shows "P xs1 xs2 xs3 xs4"
+proof -
+  let ?P = "\<lambda>xs1 xs2 xs3 xs4. P (rev xs1) (rev xs2) (rev xs3) (rev xs4)"
+  have
+    "length (rev xs1) = length (rev xs2)"
+    "length (rev xs2) = length (rev xs3)"
+    "length (rev xs3) = length (rev xs4)" using len by simp_all
+  then have "?P (rev xs1) (rev xs2) (rev xs3) (rev xs4)"
+  proof (induction rule: list_induct4)
+  qed (simp_all add: nil snoc)
+  then show "P xs1 xs2 xs3 xs4" by simp
+qed
+
+
 lemma nth_append_length_eq:
   assumes "length xs = n"
   shows "(xs @ y # zs) ! n = y"
   apply (subst nth_append) using assms by simp
 
 (* executing a list of terms (as in the call and tail-call cases) *)
-lemma compiled_list_bigstep:
+lemma compiled_arguments_bigstep:
   assumes lengths: "length vs = length ts" "length xs = length ts"
   assumes rel: "relate_exec_state f_args bs vs_arg vs_b s"
   assumes dist: "distinct xs"
@@ -140,8 +350,8 @@ lemma compiled_list_bigstep:
   assumes sem: "\<And>i s.
     \<lbrakk> i < length ts; relate_exec_state f_args bs vs_arg vs_b s \<rbrakk> \<Longrightarrow>
     \<exists>z s'. f \<turnstile> (to_imp_tc f_args crgt bs (xs ! i) keep (ts ! i), s) \<Rightarrow>\<^bsup>z\<^esup> s' \<and>
-             s' (xs ! i) = (vs ! i) \<and> s' = s on set f_args \<union> set bs \<union> set keep - {xs ! i}"
-  shows "\<exists>z s'. f \<turnstile> (t_seqs' (generate (\<lambda>i. to_imp_tc f_args crgt bs (xs ! i) keep (ts ! i)) (length ts)), s) \<Rightarrow>\<^bsup>z\<^esup> s' \<and>
+           s' (xs ! i) = (vs ! i) \<and> s' = s on set f_args \<union> set bs \<union> set keep - {xs ! i}"
+  shows "\<exists>z s'. f \<turnstile> (mk_seqs (generate (\<lambda>i. to_imp_tc f_args crgt bs (xs ! i) keep (ts ! i)) (length ts)), s) \<Rightarrow>\<^bsup>z\<^esup> s' \<and>
                 lookups xs s' = vs \<and> s' = s on set f_args \<union> set bs \<union> set keep - set xs"
 using dist keep_xs disj sem proof (induction ts xs vs rule: snoc_list_induct3)
   case Nil
@@ -161,7 +371,7 @@ next
     using that nth_append_left snoc.hyps by metis
 
   with snoc.IH[OF * **] obtain z1 s2 where exec1:
-    "f \<turnstile> (t_seqs' (generate (\<lambda>i. to_imp_tc f_args crgt bs (xs ! i) keep (ts ! i)) (length ts)), s) \<Rightarrow>\<^bsup>z1\<^esup> s2"
+    "f \<turnstile> (mk_seqs (generate (\<lambda>i. to_imp_tc f_args crgt bs (xs ! i) keep (ts ! i)) (length ts)), s) \<Rightarrow>\<^bsup>z1\<^esup> s2"
     "lookups xs s2 = vs" "s2 = s on set f_args \<union> set bs \<union> set keep - set xs"
     by blast
 
@@ -191,11 +401,11 @@ next
     [to_imp_tc f_args crgt bs ((xs @ [x]) ! length ts) keep ((ts @ [t]) ! length ts)]"
     by (simp add: generate_snoc)
 
-  have "f \<turnstile> (t_seqs' (generate (\<lambda>i. to_imp_tc f_args crgt bs (xs ! i) keep (ts ! i)) (length ts));;
+  have "f \<turnstile> (mk_seqs (generate (\<lambda>i. to_imp_tc f_args crgt bs (xs ! i) keep (ts ! i)) (length ts));;
               to_imp_tc f_args crgt bs ((xs @ [x]) ! length ts) keep ((ts @ [t]) ! length ts), s) \<Rightarrow>\<^bsup>z1 + z2\<^esup> s3"
     using exec1 exec2 by blast
-  then have *: "f \<turnstile> (t_seqs' (generate (\<lambda>i. to_imp_tc f_args crgt bs ((xs @ [x]) ! i) keep ((ts @ [t]) ! i)) (length (ts @ [t]))), s) \<Rightarrow>\<^bsup>z1 + z2\<^esup> s3"
-    using append_cs t_seqs'_t_seqs by fastforce
+  then have *: "f \<turnstile> (mk_seqs (generate (\<lambda>i. to_imp_tc f_args crgt bs ((xs @ [x]) ! i) keep ((ts @ [t]) ! i)) (length (ts @ [t]))), s) \<Rightarrow>\<^bsup>z1 + z2\<^esup> s3"
+    apply (subst append_cs ) using mk_seqs_append_bigstep sorry (* need case distinction on xs! *)
 
   have nth: "(xs @ [x]) ! length ts = x" "(vs @ [v]) ! length ts = v"
     using nth_append_length_eq snoc.hyps by metis+
@@ -214,10 +424,9 @@ qed (simp_all add: lengths)
 lemma copy_list_bigstep:
   assumes "length xs = length ys"
   assumes "distinct ys"
-  assumes "set xs \<inter> set ys = {}"
-    (* technically, these assumptions could be weakened *)
+  assumes "set xs \<inter>\<^sub>\<emptyset> set ys"
   obtains s' where
-    "f \<turnstile> (t_seqs' (generate (\<lambda>i. (ys ! i) ::= A (V (xs ! i))) (length xs)),s) \<Rightarrow>\<^bsup>Suc (2 * length xs)\<^esup> s'"
+    "f \<turnstile> (mk_seqs (generate (\<lambda>i. (ys ! i) ::= A (V (xs ! i))) (length xs)),s) \<Rightarrow>\<^bsup>Suc (2 * length xs)\<^esup> s'"
     "lookups ys s' = lookups xs s" "s' = s on (- set ys)"
 using assms proof (induction xs ys arbitrary: thesis rule: snoc_list_induct2)
   case Nil
@@ -236,17 +445,17 @@ next
     unfolding generate_def using nth_append_left snoc by fastforce
 
   from snoc obtain s2 where ih:
-      "f \<turnstile> (t_seqs' ?cs1, s) \<Rightarrow>\<^bsup>Suc (2 * length xs)\<^esup> s2"
+      "f \<turnstile> (mk_seqs ?cs1, s) \<Rightarrow>\<^bsup>Suc (2 * length xs)\<^esup> s2"
       "lookups ys s2 = lookups xs s" "s2 = s on (- set ys)"
     by auto
   moreover obtain s3 where step:
       "f \<turnstile> (?c2, s2) \<Rightarrow>\<^bsup>Suc (Suc 0)\<^esup> s3"
       "s3 y = s2 x" "s3 = s2 on (- {y})"
     by fastforce
-  ultimately have "f \<turnstile> (t_seqs' ?cs1;; ?c2, s) \<Rightarrow>\<^bsup>Suc (2 * length (xs @ [x]))\<^esup> s3" by auto
-  then have "f \<turnstile> (t_seqs' (?cs1 @ [?c2]), s) \<Rightarrow>\<^bsup>Suc (2 * length (xs @ [x]))\<^esup> s3" 
-    using t_seqs'_snoc t_seqs'_t_seqs by simp
-  then have 1: "f \<turnstile> (t_seqs' ?cs', s) \<Rightarrow>\<^bsup>Suc (2 * length (xs @ [x]))\<^esup> s3"
+  ultimately have "f \<turnstile> (mk_seqs ?cs1;; ?c2, s) \<Rightarrow>\<^bsup>Suc (2 * length (xs @ [x]))\<^esup> s3" by auto
+  then have "f \<turnstile> (mk_seqs (?cs1 @ [?c2]), s) \<Rightarrow>\<^bsup>Suc (2 * length (xs @ [x]))\<^esup> s3" 
+    (* using *) (* t_seqs'_snoc *) (* t_seqs'_t_seqs *) sorry (* need case distinction on cs1 *)
+  then have 1: "f \<turnstile> (mk_seqs ?cs', s) \<Rightarrow>\<^bsup>Suc (2 * length (xs @ [x]))\<^esup> s3"
     by (subst cs') assumption
 
   have 2: "lookups (ys @ [y]) s3 = lookups (xs @ [x]) s"
@@ -258,7 +467,7 @@ next
   from 1 2 3 snoc show ?case by blast
 qed (simp add: assms)
 
-lemma compiled_list_bigstep':
+lemma compiled_arguments_bigstep':
   assumes "length vs = length ts" "length xs = length ts"
   assumes "relate_exec_state f_args bs vs_arg vs_b s"
   assumes "distinct xs"
@@ -269,30 +478,27 @@ lemma compiled_list_bigstep':
     \<exists>z s'. f \<turnstile> (to_imp_tc f_args crgt bs (xs ! i) keep (ts ! i), s) \<Rightarrow>\<^bsup>z\<^esup> s' \<and>
              s' (xs ! i) = (vs ! i) \<and> s' = s on set f_args \<union> set bs \<union> set keep - {xs ! i}"
   obtains z s' where
-    "f \<turnstile> (t_seqs' (generate (\<lambda>i. to_imp_tc f_args crgt bs (xs ! i) keep (ts ! i)) (length ts)), s) \<Rightarrow>\<^bsup>z\<^esup> s'"
+    "f \<turnstile> (mk_seqs (generate (\<lambda>i. to_imp_tc f_args crgt bs (xs ! i) keep (ts ! i)) (length ts)), s) \<Rightarrow>\<^bsup>z\<^esup> s'"
     "lookups xs s' = vs" "s' = s on set f_args \<union> set bs \<union> set keep - set xs"
-  using compiled_list_bigstep[OF assms] by blast
+  using compiled_arguments_bigstep[OF assms] by blast
 
 lemma copy_list_bigstep':
   assumes "length xs = n"
   assumes "length ys = n"
   assumes "distinct ys"
-  assumes "set xs \<inter> set ys = {}"
+  assumes "set xs \<inter>\<^sub>\<emptyset> set ys"
   obtains s' where
-    "f \<turnstile> (t_seqs' (generate (\<lambda>i. (ys ! i) ::= A (V (xs ! i))) n),s) \<Rightarrow>\<^bsup>Suc (2 * n)\<^esup> s'"
+    "f \<turnstile> (mk_seqs (generate (\<lambda>i. (ys ! i) ::= A (V (xs ! i))) n),s) \<Rightarrow>\<^bsup>Suc (2 * n)\<^esup> s'"
     "lookups ys s' = lookups xs s" "s' = s on (- set ys)"
   using copy_list_bigstep[where xs = xs and ys = ys] assms by auto
 
 
 abbreviation "calls_r t \<equiv> set (map fst (calls t))"
 
-lemma Un_Diff_cancel1: "A \<union> B - A = B - A" for A B :: "'a set"
-  by blast
-
 theorem compiler_correct_no_tails:
   assumes "\<not> tails t"
   assumes "(f,frgt) \<turnstile> (t,vs_b,vs_arg) \<Rightarrow>\<^bsup>z\<^esup> v"
-  assumes "compiler_args_invar crgt f_args bs keep t"
+  assumes "compiler_invar crgt f_args bs keep t"
   assumes "relate_rgt_correctness frgt crgt (calls_r t)"
   assumes "relate_exec_state f_args bs vs_arg vs_b s"
   shows "\<exists>z_c s'.
@@ -303,62 +509,59 @@ using assms proof (induction t arbitrary: vs_b z v bs keep s r crgt)
   case (hLet t1 t2)
 
   let ?r1 = "fresh' (stale_registers f_args crgt bs keep LET t1 IN t2) ''Let.x''"
-  let ?t1_c = "to_imp_tc f_args crgt bs ?r1 keep t1"
-  let ?t2_c = "to_imp_tc f_args crgt (?r1 # bs) r (?r1 # keep) t2"
+  let ?c1 = "to_imp_tc f_args crgt bs ?r1 keep t1"
+  let ?c2 = "to_imp_tc f_args crgt (?r1 # bs) r (?r1 # keep) t2"
 
-  (* solve assumptions and obtain IH for t1 (and solve some assumptions for t2 at the same time, where convenient) *)
+  from hLet.prems hLet_case
+  obtain z1 v1 z2 where inv:
+      "(f, frgt) \<turnstile> (t1, vs_b, vs_arg) \<Rightarrow>\<^bsup>z1\<^esup> v1"
+      "(f, frgt) \<turnstile> (t2, v1 # vs_b, vs_arg) \<Rightarrow>\<^bsup>z2\<^esup> v"
+    by blast
 
-  have no_tails: "\<not> HOL_TCN_Timing.tails t1" "\<not> HOL_TCN_Timing.tails t2" using hLet by simp_all
+  (* solve assumptions and obtain IH for t1 *)
 
-  obtain z1 v1 z2 where
-      "z = z1 + z2" and inv: "(f, frgt) \<turnstile> (t1, vs_b, vs_arg) \<Rightarrow>\<^bsup>z1\<^esup> v1" "(f, frgt) \<turnstile> (t2, v1 # vs_b, vs_arg) \<Rightarrow>\<^bsup>z2\<^esup> v"
-    using hLet_case hLet.prems by blast
+  from hLet.prems
+  have no_tails: "\<not> HOL_TCN_Timing.tails t1" "\<not> HOL_TCN_Timing.tails t2" by simp_all
 
-  have args_invar1: "compiler_args_invar crgt f_args bs keep t1"
-    using hLet.prems compiler_args_invar_subset[where t' = "LET t1 IN t2"] by simp
+  from hLet.prems compiler_invar_let
+  have comp_invar:
+      "compiler_invar crgt f_args bs keep t1"
+      "compiler_invar crgt f_args (?r1 # bs) (?r1 # keep) t2" by auto
 
-  have rel_rgt: "relate_rgt_correctness frgt crgt (calls_r t1)" "relate_rgt_correctness frgt crgt (calls_r t2)"
-    using hLet unfolding relate_rgt_correctness_def by simp_all
+  from hLet.prems
+  have rel_rgt:
+      "relate_rgt_correctness frgt crgt (calls_r t1)"
+      "relate_rgt_correctness frgt crgt (calls_r t2)"
+    unfolding relate_rgt_correctness_def by simp_all
 
-  have rel_state1: "relate_exec_state f_args bs vs_arg vs_b s" using hLet by blast
+  from hLet.prems have rel_state1: "relate_exec_state f_args bs vs_arg vs_b s" by blast
 
   obtain z1_c s2 where ih1:
-      "f_c \<turnstile> (?t1_c, s) \<Rightarrow>\<^bsup>z1_c\<^esup> s2" "s2 ?r1 = v1" "s2 = s on set f_args \<union> set bs \<union> set keep - {?r1}"
-    using hLet.IH(1) no_tails(1) inv(1) args_invar1 rel_rgt(1) rel_state1 by blast
+      "f_c \<turnstile> (?c1, s) \<Rightarrow>\<^bsup>z1_c\<^esup> s2" "s2 ?r1 = v1" "s2 = s on set f_args \<union> set bs \<union> set keep - {?r1}"
+    using hLet.IH(1) no_tails(1) inv(1) comp_invar(1) rel_rgt(1) rel_state1 by blast
 
   (* solve assumptions and obtain IH for t2 *)
 
-  have "?r1 \<notin> set f_args"
-    apply (rule contra_subsetD[OF _ fresh_not_in_stale])
-    unfolding stale_registers_def by simp
-  moreover have "?r1 \<notin> set (call_registers crgt t2)"
-    apply (rule contra_subsetD[OF _ fresh_not_in_stale])
-    using call_registers_set unfolding stale_registers_def by auto
-  moreover have "compiler_args_invar crgt f_args bs keep t2"
-    using hLet.prems compiler_args_invar_subset[where t' = "LET t1 IN t2"] by simp
-  ultimately have args_invar2: "compiler_args_invar crgt f_args (?r1 # bs) (?r1 # keep) t2"
-    using hLet.prems(3) unfolding compiler_args_invar_def by auto
-
-  have s_like_s2: "s2 = s on set f_args \<union> set bs \<union> set keep" (* TODO *)
-    by (smt (verit) DiffI Un_iff eq_on_def fresh_not_in_stale ih1(3) set_append singletonD stale_registers_def)
+  have s2_like_s: "s2 = s on set f_args \<union> set bs \<union> set keep" (* TODO *)
+    by (metis Diff_empty Diff_insert0 Un_iff fresh_not_in_stale ih1(3) set_append stale_registers_def)
   then have rel_state2: "relate_exec_state f_args (?r1 # bs) vs_arg (v1 # vs_b) s2"
-    using hLet.prems(5) unfolding relate_exec_state_def using ih1 by fastforce
+    using hLet.prems unfolding relate_exec_state_def using ih1 by fastforce
 
   obtain z2_c s3 where ih2:
-      "f_c \<turnstile> (?t2_c, s2) \<Rightarrow>\<^bsup>z2_c\<^esup>  s3" "s3 r = v"
+      "f_c \<turnstile> (?c2, s2) \<Rightarrow>\<^bsup>z2_c\<^esup>  s3" "s3 r = v"
       "s3 = s2 on set f_args \<union> set (?r1 # bs) \<union> set (?r1 # keep) - {r}"
-    using hLet.IH(2) no_tails(2) inv(2) args_invar2 rel_rgt(2) rel_state2 by blast
+    using hLet.IH(2) no_tails(2) inv(2) comp_invar(2) rel_rgt(2) rel_state2 by blast
 
   (* put it together *)
 
-  have s2_like_s3: "s3 = s2 on set f_args \<union> set bs \<union> set keep - {r}"
+  have "s3 = s2 on set f_args \<union> set bs \<union> set keep - {r}"
     using Un_Diff ih2(3) by auto
-  with s_like_s2 have s_like_s3: "s3 = s on set f_args \<union> set bs \<union> set keep - {r}"
+  with s2_like_s have "s3 = s on set f_args \<union> set bs \<union> set keep - {r}"
     by (simp add: eq_on_def)
 
-  show ?case
+  then show ?case
     unfolding to_imp_tc.simps Let_def
-    using ih1 ih2 s_like_s3 by blast
+    using ih1 ih2 by blast
 next
   case (hLetBound n)
   show ?case
@@ -389,76 +592,84 @@ next
   case (hIf t1 t2 t3)
 
   let ?r1 = "fresh' (stale_registers f_args crgt bs keep (IF t1\<noteq>0 THEN t2 ELSE t3)) ''If.x''"
+  let ?c1 = "to_imp_tc f_args crgt bs ?r1 keep t1"
+  let ?c2 = "to_imp_tc f_args crgt bs r keep t2"
+  let ?c3 = "to_imp_tc f_args crgt bs r keep t3"
 
-  have no_tails: "\<not> HOL_TCN_Timing.tails t1" "\<not> HOL_TCN_Timing.tails t2" "\<not> HOL_TCN_Timing.tails t3" using hIf by simp_all
-  then have "invar t1" "invar t2" "invar t3" by simp_all
-  then have args_invar:
-      "compiler_args_invar crgt f_args bs keep t1"
-      "compiler_args_invar crgt f_args bs keep t2"
-      "compiler_args_invar crgt f_args bs keep t3"
-    using hIf.prems compiler_args_invar_subset[where t = t1 and t' = "IF t1\<noteq>0 THEN t2 ELSE t3"] apply simp
-    using hIf.prems compiler_args_invar_subset[where t = t2 and t' = "IF t1\<noteq>0 THEN t2 ELSE t3"] apply fastforce
-    using hIf.prems compiler_args_invar_subset[where t = t3 and t' = "IF t1\<noteq>0 THEN t2 ELSE t3"] apply fastforce (* TODO ? *)
-    done
+  from hIf.prems
+  have no_tails:
+    "\<not> HOL_TCN_Timing.tails t1"
+    "\<not> HOL_TCN_Timing.tails t2"
+    "\<not> HOL_TCN_Timing.tails t3" by simp_all
 
-  have rel_rgt: "relate_rgt_correctness frgt crgt (calls_r t1)" "relate_rgt_correctness frgt crgt (calls_r t2)" "relate_rgt_correctness frgt crgt (calls_r t3)"
-    using hIf unfolding relate_rgt_correctness_def by simp_all
+  from compiler_invar_if[OF hIf.prems(3)]
+  have comp_invar:
+      "compiler_invar crgt f_args bs keep t1"
+      "compiler_invar crgt f_args bs keep t2"
+      "compiler_invar crgt f_args bs keep t3" by auto
 
-  have rel_state1: "relate_exec_state f_args bs vs_arg vs_b s" using hIf by blast
+  from hIf.prems
+  have rel_rgt:
+      "relate_rgt_correctness frgt crgt (calls_r t1)"
+      "relate_rgt_correctness frgt crgt (calls_r t2)"
+      "relate_rgt_correctness frgt crgt (calls_r t3)"
+    unfolding relate_rgt_correctness_def by simp_all
+
+  from hIf.prems have rel_state1: "relate_exec_state f_args bs vs_arg vs_b s" by blast
 
   show ?case
   proof (cases rule: hIf_case[OF hIf.prems(2)])
-    case (1 z1 v1 z2)
+    case ifTrue: (1 z1 v1 z2)
 
     obtain z1_c s2 where ih1:
-        "f_c \<turnstile> (to_imp_tc f_args crgt bs ?r1 keep t1, s) \<Rightarrow>\<^bsup>z1_c\<^esup> s2"
+        "f_c \<turnstile> (?c1, s) \<Rightarrow>\<^bsup>z1_c\<^esup> s2"
         "s2 ?r1 = v1" "s2 = s on set f_args \<union> set bs \<union> set keep - {?r1}"
-      using hIf.IH(1) no_tails(1) 1 args_invar(1) rel_rgt(1) rel_state1 by blast
+      using hIf.IH(1) no_tails(1) ifTrue comp_invar(1) rel_rgt(1) rel_state1 by blast
 
-    have s_like_s2: "s2 = s on set f_args \<union> set bs \<union> set keep" (* TODO *)
-      by (smt (verit) DiffI Un_iff eq_on_def fresh_not_in_stale ih1(3) set_append singletonD stale_registers_def)
+    have s2_like_s: "s2 = s on set f_args \<union> set bs \<union> set keep" (* TODO *)
+      by (metis Diff_empty Diff_insert0 Un_iff fresh_not_in_stale ih1(3) set_append stale_registers_def)
     then have rel_state2: "relate_exec_state f_args bs vs_arg vs_b s2"
-      using hIf.prems(5) unfolding relate_exec_state_def using ih1 by fastforce
+      using hIf.prems unfolding relate_exec_state_def using ih1 by fastforce
 
     obtain z2_c s3 where ih2:
-        "f_c \<turnstile> (to_imp_tc f_args crgt bs r keep t2, s2) \<Rightarrow>\<^bsup>z2_c\<^esup>  s3" "s3 r = v"
+        "f_c \<turnstile> (?c2, s2) \<Rightarrow>\<^bsup>z2_c\<^esup>  s3" "s3 r = v"
         "s3 = s2 on set f_args \<union> set bs \<union> set keep - {r}"
-      using hIf.IH(2) no_tails(2) 1 args_invar(2) rel_rgt(2) rel_state2 by blast
+      using hIf.IH(2) no_tails(2) ifTrue comp_invar(2) rel_rgt(2) rel_state2 by blast
   
-    have s2_like_s3: "s3 = s2 on set f_args \<union> set bs \<union> set keep - {r}"
+    have "s3 = s2 on set f_args \<union> set bs \<union> set keep - {r}"
       using Un_Diff ih2(3) by auto
-    with s_like_s2 have s_like_s3: "s3 = s on set f_args \<union> set bs \<union> set keep - {r}"
+    with s2_like_s have "s3 = s on set f_args \<union> set bs \<union> set keep - {r}"
       by (simp add: eq_on_def)
   
-    show ?thesis
+    then show ?thesis
       unfolding to_imp_tc.simps Let_def
-      using ih1 ih2 s_like_s3 1 by blast
+      using ih1 ih2 ifTrue by blast
   next
-    case (2 z1 z2)
+    case ifFalse: (2 z1 z2)
 
     obtain z1_c s2 where ih1:
-        "f_c \<turnstile> (to_imp_tc f_args crgt bs ?r1 keep t1, s) \<Rightarrow>\<^bsup>z1_c\<^esup> s2"
+        "f_c \<turnstile> (?c1, s) \<Rightarrow>\<^bsup>z1_c\<^esup> s2"
         "s2 ?r1 = 0" "s2 = s on set f_args \<union> set bs \<union> set keep - {?r1}"
-      using hIf.IH(1) no_tails(1) 2(2) args_invar(1) rel_rgt(1) rel_state1 by metis
+      using hIf.IH(1) no_tails(1) ifFalse comp_invar(1) rel_rgt(1) rel_state1 by metis
 
-    have s_like_s2: "s2 = s on set f_args \<union> set bs \<union> set keep" (* TODO *)
-      by (smt (verit) DiffI Un_iff eq_on_def fresh_not_in_stale ih1(3) set_append singletonD stale_registers_def)
+    have s2_like_s: "s2 = s on set f_args \<union> set bs \<union> set keep" (* TODO *)
+      by (metis Diff_empty Diff_insert0 Un_iff fresh_not_in_stale ih1(3) set_append stale_registers_def)
     then have rel_state3: "relate_exec_state f_args bs vs_arg vs_b s2"
       using hIf.prems(5) unfolding relate_exec_state_def using ih1 by fastforce
 
     obtain z2_c s3 where ih3:
-        "f_c \<turnstile> (to_imp_tc f_args crgt bs r keep t3, s2) \<Rightarrow>\<^bsup>z2_c\<^esup>  s3" "s3 r = v"
+        "f_c \<turnstile> (?c3, s2) \<Rightarrow>\<^bsup>z2_c\<^esup>  s3" "s3 r = v"
         "s3 = s2 on set f_args \<union> set bs \<union> set keep - {r}"
-      using hIf.IH(3) no_tails(3) 2 args_invar(3) rel_rgt(3) rel_state3 by blast
+      using hIf.IH(3) no_tails(3) ifFalse comp_invar(3) rel_rgt(3) rel_state3 by blast
   
-    have s2_like_s3: "s3 = s2 on set f_args \<union> set bs \<union> set keep - {r}"
+    have "s3 = s2 on set f_args \<union> set bs \<union> set keep - {r}"
       using Un_Diff ih3(3) by auto
-    with s_like_s2 have s_like_s3: "s3 = s on set f_args \<union> set bs \<union> set keep - {r}"
+    with s2_like_s have "s3 = s on set f_args \<union> set bs \<union> set keep - {r}"
       by (simp add: eq_on_def)
   
-    show ?thesis
+    then show ?thesis
       unfolding to_imp_tc.simps Let_def
-      using ih1 ih3 s_like_s3 2 by blast
+      using ih1 ih3 ifFalse by blast
   qed
 next
   case (hCall gr ts)
@@ -466,19 +677,18 @@ next
   let ?g = "f_from_frgt frgt gr"
   let ?T_g = "T_f_from_frgt frgt gr"
 
+  from hCall.prems hCall_case
   obtain zs vs where
           z: "z = sum_list zs + ?T_g vs"
       and lengths: "length zs = length ts" "length vs = length ts"
       and args_bigstep: "\<forall>i<length ts. (f, frgt) \<turnstile> (ts ! i, vs_b, vs_arg) \<Rightarrow>\<^bsup>zs ! i\<^esup> vs ! i"
       and gvs: "?g vs = v"
-    using hCall_case hCall split_from_frgt by auto
-
+    using split_from_frgt by auto
 
   (* part 1: computing the arguments *)
 
   let ?xs = "make_n_fresh (stale_registers f_args crgt bs keep (hCall gr ts)) ''Call.x.'' (length ts)"
-  let ?c1 = "t_seqs' (generate (\<lambda>i. to_imp_tc f_args crgt bs (?xs ! i) (?xs @ keep) (ts ! i)) (length ts))"
-
+  let ?c1 = "mk_seqs (generate (\<lambda>i. to_imp_tc f_args crgt bs (?xs ! i) (?xs @ keep) (ts ! i)) (length ts))"
 
   have "length vs = length ts" "length ?xs = length ts"
     using lengths unfolding make_n_fresh_def generate_def by simp_all
@@ -487,26 +697,21 @@ next
   moreover have "set ?xs \<subseteq> set (?xs @ keep)" by simp
   moreover have "set f_args \<inter>\<^sub>\<emptyset> set ?xs" "set bs \<inter>\<^sub>\<emptyset> set ?xs"
     unfolding stale_registers_def using make_n_fresh_not_in_stale by fastforce+
-  moreover have "\<exists>z_c s'. f_c \<turnstile> (to_imp_tc f_args crgt bs (?xs ! i) (?xs @ keep) (ts ! i), s) \<Rightarrow>\<^bsup>z_c\<^esup>  s' \<and>
-       s' (?xs ! i) = (vs ! i) \<and> s' = s on set f_args \<union> set bs \<union> set (?xs @ keep) - {?xs ! i}"
+  moreover have
+      "\<exists>z_c s'. f_c \<turnstile> (to_imp_tc f_args crgt bs (?xs ! i) (?xs @ keep) (ts ! i), s) \<Rightarrow>\<^bsup>z_c\<^esup>  s' \<and>
+                s' (?xs ! i) = (vs ! i) \<and> s' = s on set f_args \<union> set bs \<union> set (?xs @ keep) - {?xs ! i}"
     if "i < length ts" "relate_exec_state f_args bs vs_arg vs_b s" for i s
   proof (rule hCall.IH)
     from that show "ts ! i \<in> set ts" by simp
   next
-    from that hCall.prems(1) show "\<not> HOL_TCN_Timing.tails (ts ! i)" by simp
+    from that hCall.prems
+    show "\<not> HOL_TCN_Timing.tails (ts ! i)" by simp
   next
-    from that args_bigstep show "(f, frgt) \<turnstile> (ts ! i, vs_b, vs_arg) \<Rightarrow>\<^bsup>zs ! i\<^esup>  vs ! i" by simp
+    from that args_bigstep
+    show "(f, frgt) \<turnstile> (ts ! i, vs_b, vs_arg) \<Rightarrow>\<^bsup>zs ! i\<^esup>  vs ! i" by simp
   next
-    have "set (call_registers crgt (ts ! i)) \<subseteq> set (call_registers crgt (hCall gr ts))"
-      using call_registers_set that by fastforce
-    then have "set ?xs \<inter>\<^sub>\<emptyset> set (call_registers crgt (ts ! i))"
-      unfolding stale_registers_def using lengths make_n_fresh_not_in_stale by fastforce
-    moreover have "set ?xs \<inter>\<^sub>\<emptyset> set f_args"
-      unfolding stale_registers_def using make_n_fresh_not_in_stale by fastforce
-    moreover from that have "compiler_args_invar crgt f_args bs keep (ts ! i)"
-      using hCall.prems(1,3) compiler_args_invar_subset[where t = "ts ! i" and t' = "hCall gr ts"] by fastforce
-    ultimately show "compiler_args_invar crgt f_args bs (?xs @ keep) (ts ! i)"
-      unfolding compiler_args_invar_def by auto
+    from that hCall.prems compiler_invar_call
+    show "compiler_invar crgt f_args bs (?xs @ keep) (ts ! i)" by simp
   next
     from that show "relate_rgt_correctness frgt crgt (calls_r (ts ! i))"
       using hCall.prems(4) unfolding relate_rgt_correctness_def by fastforce
@@ -516,29 +721,27 @@ next
 
   ultimately obtain z1 s2 where exec_c1: "f_c \<turnstile> (?c1, s) \<Rightarrow>\<^bsup>z1\<^esup>  s2"
       "lookups ?xs s2 = vs" "s2 = s on set f_args \<union> set bs \<union> set (?xs @ keep) - set ?xs"
-    using compiled_list_bigstep' by blast
-
+    using compiled_arguments_bigstep' by blast
 
   (* part 2: copying from temporaries to argument registers *)
 
-  let ?c2 = "t_seqs' (generate (\<lambda>i. (args_from_crgt crgt gr ! i) ::= A (V (?xs ! i))) (length ts))"
+  let ?c2 = "mk_seqs (generate (\<lambda>i. (args_from_crgt crgt gr ! i) ::= A (V (?xs ! i))) (length ts))"
   let ?z2 = "Suc (2 * length ts)"
 
   have "set (args_from_crgt crgt gr) \<subseteq> set (stale_registers f_args crgt bs keep (hCall gr ts))"
-    unfolding stale_registers_def call_registers_def by fastforce
-  then have dj: "set ?xs \<inter> set (args_from_crgt crgt gr) = {}"
+    unfolding stale_registers_def call_registers_def using calls'_set by auto
+  then have "set ?xs \<inter>\<^sub>\<emptyset> set (args_from_crgt crgt gr)"
     using make_n_fresh_not_in_stale by blast
   moreover have "distinct (args_from_crgt crgt gr)"
-    using hCall.prems unfolding compiler_args_invar_def by simp
+    using hCall.prems unfolding compiler_invar_def calls'_set by simp
   moreover have "length ?xs = length ts"
     unfolding make_n_fresh_def generate_def by simp
   moreover have "length (args_from_crgt crgt gr) = length ts"
-    using hCall.prems unfolding compiler_args_invar_def by simp
+    using hCall.prems unfolding compiler_invar_def calls_n_set by simp
 
   ultimately obtain s3 where exec_c2: "f_c \<turnstile> (?c2, s2) \<Rightarrow>\<^bsup>?z2\<^esup> s3"
        "lookup_args crgt gr s3 = lookups ?xs s2" "s3 = s2 on - set (args_from_crgt crgt gr)"
     using copy_list_bigstep' by blast
-                       
 
   (* part 3: calling g *)
   
@@ -554,7 +757,6 @@ next
   have "f_from_frgt frgt gr = ?g" using split_from_frgt by simp
   then have vfrom: "?gv = v" using exec_c1(2) exec_c2(2) gvs by simp
 
-
   (* part 4: copying to r *)
 
   let ?c4 = "r ::= A (V (ret_from_crgt crgt gr)) :: tcom"
@@ -562,7 +764,6 @@ next
   let ?s5 = "?s4(r := aval (A (V ?gret)) ?s4)"
   obtain z4 where exec_c4: "f_c \<turnstile> (?c4, ?s4) \<Rightarrow>\<^bsup>z4\<^esup> ?s5" by blast
   then have s5: "?s5 = ?s4(r := v)" using vfrom exec_c3 by simp
-
 
   (* putting it together *)
 
@@ -580,12 +781,12 @@ next
       using exec_c1 by blast
 
     have "set f_args \<union> set bs \<union> set keep \<inter>\<^sub>\<emptyset> set (args_from_crgt crgt gr)"
-      using hCall.prems(3) unfolding compiler_args_invar_def call_registers_def by auto
+      using hCall.prems(3) unfolding compiler_invar_def call_registers_def using calls'_set by auto
     then have **: "s3 = s2 on set f_args \<union> set bs \<union> set keep - {r}"
-      using hCall.prems(3) exec_c2 unfolding compiler_args_invar_def by auto
+      using hCall.prems(3) exec_c2 unfolding compiler_invar_def by auto
 
     have "ret_from_crgt crgt gr \<notin> set f_args \<union> set bs \<union> set keep"
-      using hCall.prems(3) unfolding compiler_args_invar_def call_registers_def by auto
+      using hCall.prems(3) unfolding compiler_invar_def call_registers_def using calls'_set by auto
     then have ***: "?s5 = s3 on set f_args \<union> set bs \<union> set keep - {r}" by auto
 
     show "?s5 = s on set f_args \<union> set bs \<union> set keep - {r}"
@@ -597,59 +798,215 @@ next
   then show ?case by simp
 qed
 
+(* In the compiled trace relatedness proof, we frequently apply the IH to obtain relatedness
+   theorems for subterms (assumption comp_rel). By using the theorems relating traces and bigstep
+   semantics, we can add the compiler correctness results for the execution of those subterms.
+   Those we need to continue applying the IH to further subterms, e.g. the IH for the second
+   LET subterm requires a well-formed starting state. *)
+lemma compiler_augment_rel_trace:
+  assumes no_tails: "\<not> HOL_TCN_Timing.tails t"
+  assumes htrace: "frgt \<turnstile> (t,vs_b,vs_arg) \<Rightarrow>\<^bsup> hT :: HOL_TCN_Timing.trace \<^esup> Value v"
+  assumes comp_assms:
+    "compiler_invar crgt f_args bs keep t"
+    and "relate_rgt_correctness frgt crgt (calls_r t)"
+    and "relate_exec_state f_args bs vs_arg vs_b s"
+  assumes comp_rel:
+    "(to_imp_tc f_args crgt bs r keep t,s) \<Rightarrow>\<^bsup>(k, cT)\<^esup> (s', False)"
+    and "rel_trace_to_leaf crgt f_args r hT (Value v) cT s' False"
+  shows "s' r = v" "s' = s on set f_args \<union> set bs \<union> set keep - {r}"
+proof -
+  from assms trace_val_to_semantics
+  obtain f z where "(f,frgt) \<turnstile> (t,vs_b,vs_arg) \<Rightarrow>\<^bsup>z\<^esup> v" by blast
 
+  then obtain f_c z_c s2 where correct:
+      "f_c \<turnstile> (to_imp_tc f_args crgt bs r keep t,s) \<Rightarrow>\<^bsup>z_c\<^esup> s2" "s2 r = v"
+      "s2 = s on set f_args \<union> set bs \<union> set keep - {r}"
+    using compiler_correct_no_tails[where t = t] assms by blast
 
-definition rel_trace_call :: "com_registry \<Rightarrow> fun_ref \<Rightarrow> nat list \<Rightarrow> com \<Rightarrow> state \<Rightarrow> bool" where
-  "rel_trace_call crgt gr gargs gcom gs \<longleftrightarrow> com_from_crgt crgt gr = gcom \<and> lookup_args crgt gr gs = gargs"
-definition rel_trace_calls :: "com_registry \<Rightarrow> HOL_TCN_Timing.trace \<Rightarrow> IMP_Tailcall_Traces.call_trace \<Rightarrow> bool" where
-  "rel_trace_calls crgt hT cT \<longleftrightarrow>
-    length hT = length cT \<and>
-    list_all (\<lambda>((gr,gargs),(gcom,gs)). rel_trace_call crgt gr gargs gcom gs) (zip hT cT)"
-(* "rel_trace_calls crgt hT cT \<longleftrightarrow>
-    length hT = length cT \<and>
-    (\<forall>i < length hT. let (gr, gargs) = hT ! i; (gcom, gs) = cT ! i in
-                     rel_trace_call crgt gr gargs gcom gs)" *)
-fun rel_leaf_state :: "com_registry \<Rightarrow> vname list \<Rightarrow> vname \<Rightarrow> leaf_state \<Rightarrow> state \<Rightarrow> bool \<Rightarrow> bool" where
-  "rel_leaf_state crgt _      r (Value v) s l \<longleftrightarrow> \<not> l \<and> s       r        = v " |
-  "rel_leaf_state crgt f_args _ (Tail vs) s l \<longleftrightarrow>   l \<and> lookups f_args s = vs"
+  have "s2 = s'" using correct(1) trace_nontail_has_bigstep[OF comp_rel(1)] determ(2) by blast
 
-definition rel_trace_to_leaf ::
-    "com_registry \<Rightarrow> vname list \<Rightarrow> vname \<Rightarrow>
-      HOL_TCN_Timing.trace \<Rightarrow> leaf_state \<Rightarrow>
-        IMP_Tailcall_Traces.call_trace \<Rightarrow> state \<Rightarrow> bool \<Rightarrow> bool" where
-  "rel_trace_to_leaf crgt f_args r hT hl cT s cl \<longleftrightarrow>
-    rel_trace_calls crgt hT cT \<and> rel_leaf_state crgt f_args r hl s cl"
+  then show "s' r = v" "s' = s on set f_args \<union> set bs \<union> set keep - {r}" using correct by simp_all
+qed
 
-(* lemma
+(* executing a list of terms (as in the call and tail-call cases) *)
+lemma compiled_arguments_trace:
+  assumes lengths: "length vs = length ts" "length xs = length ts" "length hTs = length ts"
+  assumes rel: "relate_exec_state f_args bs vs_arg vs_b s"
+  assumes args: "distinct xs" "set xs \<subseteq> set keep" "set f_args \<inter>\<^sub>\<emptyset> set xs" "set bs \<inter>\<^sub>\<emptyset> set xs"
+  assumes trace: "\<And>i. i < length ts \<Longrightarrow> frgt \<turnstile> (ts ! i, vs_b, vs_arg) \<Rightarrow>\<^bsup>hTs ! i\<^esup>  Value (vs ! i)"
+  assumes sem: "\<And>i s.
+    \<lbrakk> i < length ts; relate_exec_state f_args bs vs_arg vs_b s \<rbrakk> \<Longrightarrow>
+    \<exists>k cT s'. (to_imp_tc f_args crgt bs (xs ! i) keep (ts ! i), s) \<Rightarrow>\<^bsup>(k, cT)\<^esup>  (s', False) \<and>
+              rel_trace_to_leaf crgt f_args (xs ! i) (hTs ! i) (Value (vs ! i)) cT s' False \<and>
+              s' (xs ! i) = (vs ! i) \<and> s' = s on set f_args \<union> set bs \<union> set keep - {xs ! i}"
+  shows "\<exists>k cT s'. (mk_seqs (generate (\<lambda>i. to_imp_tc f_args crgt bs (xs ! i) keep (ts ! i)) (length ts)), s) \<Rightarrow>\<^bsup>(k, cT)\<^esup> (s', False) \<and>
+                   rel_trace_calls crgt (concat hTs) cT \<and>
+                   lookups xs s' = vs \<and> s' = s on set f_args \<union> set bs \<union> set keep - set xs"
+using args trace sem proof (induction ts xs vs hTs rule: snoc_list_induct4)
+  case Nil
+  then show ?case unfolding generate_def rel_trace_calls_def using ttrace_to_leaf.tSkip by auto
+next
+  case (snoc ts t xs x vs v hTs hT)
+
+  (* obtain the IH *)
+  have *: "i < length (ts @ [t])" if "i < length ts" for i using that by simp
+
+  from snoc have "distinct xs" "set xs \<subseteq> set keep" "set f_args \<inter>\<^sub>\<emptyset> set xs" "set bs \<inter>\<^sub>\<emptyset> set xs" by simp_all
+  moreover from * snoc.prems have "frgt \<turnstile> (ts ! i, vs_b, vs_arg) \<Rightarrow>\<^bsup>hTs ! i\<^esup>  Value (vs ! i)" if "i < length ts" for i
+    using that nth_append_left snoc.hyps by metis
+  moreover from * snoc.prems have "\<exists>k cT s'.
+        (to_imp_tc f_args crgt bs (xs ! i) keep (ts ! i), s) \<Rightarrow>\<^bsup>(k, cT)\<^esup>  (s', False) \<and>
+        rel_trace_to_leaf crgt f_args (xs ! i) (hTs ! i) (Value (vs ! i)) cT s' False \<and>
+        s' (xs ! i) = (vs ! i) \<and> s' = s on set f_args \<union> set bs \<union> set keep - {xs ! i}"
+      if "i < length ts" "relate_exec_state f_args bs vs_arg vs_b s" for i s
+    using that nth_append_left snoc.hyps by metis
+
+  ultimately obtain k1 cT1 s2 where trace1:
+      "(mk_seqs (generate (\<lambda>i. to_imp_tc f_args crgt bs (xs ! i) keep (ts ! i)) (length ts)), s) \<Rightarrow>\<^bsup>(k1, cT1)\<^esup>  (s2, False)"
+      "rel_trace_calls crgt (concat hTs) cT1"
+      "lookups xs s2 = vs" "s2 = s on set f_args \<union> set bs \<union> set keep - set xs"
+    using snoc.IH by blast
+
+  (* obtain the step *)
+
+  have *: "length ts < length (ts @ [t])" by simp
+
+  from rel trace1(4) snoc.prems(3,4) have **: "relate_exec_state f_args bs vs_arg vs_b s2"
+    unfolding relate_exec_state_def by fastforce
+
+  from * ** snoc.prems(6)
+  obtain k2 cT2 s3 where trace2:
+      "(to_imp_tc f_args crgt bs ((xs @ [x]) ! length ts) keep ((ts @ [t]) ! length ts), s2) \<Rightarrow>\<^bsup>(k2, cT2)\<^esup>  (s3, False)"
+      "rel_trace_to_leaf crgt f_args ((xs @ [x]) ! length ts) ((hTs @ [hT]) ! length ts) (Value ((vs @ [v]) ! length ts)) cT2 s3 False"
+      "s3 ((xs @ [x]) ! length ts) = (vs @ [v]) ! length ts"
+      "s3 = s2 on set f_args \<union> set bs \<union> set keep - {(xs @ [x]) ! length ts}"
+    by blast
+
+  (* put it together *)
+
+  have nth: "(xs @ [x]) ! length ts = x" "(vs @ [v]) ! length ts = v" "(hTs @ [hT]) ! length ts = hT"
+    using nth_append_length_eq snoc.hyps by metis+
+
+  show ?case
+  proof (repeat \<open>rule exI\<close>, repeat \<open>rule conjI\<close>)
+
+    have "(xs @ [x]) ! i = xs ! i" "(ts @ [t]) ! i = ts ! i" if "i < length ts" for i
+      using nth_append_left snoc.hyps that by metis+
+    then have "generate (\<lambda>i. to_imp_tc f_args crgt bs (xs ! i) keep (ts ! i)) (length ts) =
+        generate (\<lambda>i. to_imp_tc f_args crgt bs ((xs @ [x]) ! i) keep ((ts @ [t]) ! i)) (length ts)"
+      unfolding generate_def by simp
+    then have append_cs:
+        "generate (\<lambda>i. to_imp_tc f_args crgt bs ((xs @ [x]) ! i) keep ((ts @ [t]) ! i)) (length (ts @ [t])) =
+         generate (\<lambda>i. to_imp_tc f_args crgt bs (xs ! i) keep (ts ! i)) (length ts) @
+         [to_imp_tc f_args crgt bs ((xs @ [x]) ! length ts) keep ((ts @ [t]) ! length ts)]"
+      by (simp add: generate_snoc)
+  
+    have "(mk_seqs (generate (\<lambda>i. to_imp_tc f_args crgt bs (xs ! i) keep (ts ! i)) (length ts));;
+                to_imp_tc f_args crgt bs ((xs @ [x]) ! length ts) keep ((ts @ [t]) ! length ts), s) \<Rightarrow>\<^bsup>(k1 + k2, cT1 @ cT2)\<^esup> (s3,False)"
+      using trace1 trace2 ttrace_to_leaf.tSeq by blast
+    then show "(mk_seqs (generate (\<lambda>i. to_imp_tc f_args crgt bs ((xs @ [x]) ! i) keep ((ts @ [t]) ! i)) (length (ts @ [t]))), s) \<Rightarrow>\<^bsup>(k1 + k2, cT1 @ cT2)\<^esup> (s3,False)"
+      using append_cs (* t_seqs'_t_seqs *) sorry
+  next
+    show "rel_trace_calls crgt (concat (hTs @ [hT])) (cT1 @ cT2)"
+      using rel_trace_calls_append trace1(2) trace2(2)[simplified rel_trace_to_leaf_def nth] by simp
+  next
+    from trace2(3) have "s3 x = v" using snoc.hyps nth_append_length by metis
+    moreover from trace2(4) nth(1) snoc.prems(1,2) have "s3 = s2 on set xs" by auto
+    ultimately show "lookups (xs @ [x]) s3 = vs @ [v]" using trace1(3) by auto
+  next
+    show "s3 = s on set f_args \<union> set bs \<union> set keep - set (xs @ [x])"
+      using nth trace1(4) trace2(4) by auto
+  qed
+
+qed (simp_all add: lengths)
+
+(* copying a list of registers *)
+lemma copy_list_trace:
   assumes "length xs = length ys"
-  shows "(\<forall>i<length xs. P (xs ! i) (ys ! i)) = list_all (\<lambda>(x, y). P x y) (zip xs ys)"
-   apply (induction rule: snoc_list_induct2[OF assms])  *)
+  assumes "distinct ys"
+  assumes "set xs \<inter>\<^sub>\<emptyset> set ys"
+  obtains s' where
+    "(mk_seqs (generate (\<lambda>i. (ys ! i) ::= A (V (xs ! i))) (length xs)),s) \<Rightarrow>\<^bsup>(Suc (2 * length xs), [])\<^esup> (s', False)"
+    "lookups ys s' = lookups xs s" "s' = s on (- set ys)"
+using assms proof (induction xs ys arbitrary: thesis rule: snoc_list_induct2)
+  case Nil
+  then show ?case unfolding generate_def using ttrace_to_leaf.tSkip by auto
+next
+  case (snoc xs x ys y)
 
-lemma rel_trace_append:
-  assumes "rel_trace_calls crgt hT1 cT1"
-  assumes "rel_trace_to_leaf crgt f_args r hT2 hl cT2 s cl"
-  shows "rel_trace_to_leaf crgt f_args r (hT1 @ hT2) hl (cT1 @ cT2) s cl"
-  using assms unfolding rel_trace_to_leaf_def rel_trace_calls_def by auto
+  let ?cs = "\<lambda>xs ys. generate (\<lambda>i. (ys ! i) ::= A (V (xs ! i)) :: tcom) (length xs)"
 
+  let ?cs1 = "?cs xs ys"
+  let ?c2 = "y ::= A (V x) :: tcom"
+  let ?cs' = "?cs (xs @ [x]) (ys @ [y])"
 
-term "undefined :: HOL_TCN_Timing.trace"
-term "undefined :: IMP_Tailcall_Traces.trace"
-term htrace_to_leaf
-term ttrace_to_leaf
+  have cs': "?cs' = ?cs1 @ [?c2]"
+    apply (simp add: generate_snoc)
+    unfolding generate_def using nth_append_left snoc by fastforce
 
+  from snoc obtain s2 where ih:
+      "(mk_seqs ?cs1, s) \<Rightarrow>\<^bsup>(Suc (2 * length xs), [])\<^esup> (s2,False)"
+      "lookups ys s2 = lookups xs s" "s2 = s on (- set ys)"
+    by auto
+  moreover obtain s3 where step:
+      "(?c2, s2) \<Rightarrow>\<^bsup>(Suc (Suc 0), [])\<^esup> (s3, False)"
+      "s3 y = s2 x" "s3 = s2 on (- {y})"
+    using ttrace_to_leaf.tAssign by fastforce
+  ultimately have "(mk_seqs ?cs1;; ?c2, s) \<Rightarrow>\<^bsup>(Suc (2 * length (xs @ [x])), [])\<^esup> (s3,False)"
+    using ttrace_to_leaf.tSeq by auto
+  then have "(mk_seqs (?cs1 @ [?c2]), s) \<Rightarrow>\<^bsup>(Suc (2 * length (xs @ [x])), [])\<^esup> (s3,False)" 
+    (* using (* t_seqs'_snoc *) t_seqs'_t_seqs *) sorry
+  then have 1: "(mk_seqs ?cs', s) \<Rightarrow>\<^bsup>(Suc (2 * length (xs @ [x])), [])\<^esup> (s3,False)"
+    by (subst cs') assumption
 
-thm compiler_correct_no_tails
-thm trace_val_to_semantics
+  have "s3 = s2 on set ys" using snoc step by auto
+  then have "lookups ys s3 = lookups ys s2" by auto
+  then have 2: "lookups (ys @ [y]) s3 = lookups (xs @ [x]) s"
+    using ih step snoc by auto
+
+  have 3: "s3 = s on (- set (ys @ [y]))"
+    using ih step by auto
+
+  from 1 2 3 snoc show ?case by blast
+qed (simp add: assms)
+
+lemma compiled_arguments_trace':
+  assumes lengths: "length vs = length ts" "length xs = length ts" "length hTs = length ts"
+  assumes rel: "relate_exec_state f_args bs vs_arg vs_b s"
+  assumes dist: "distinct xs"
+  assumes keep_xs: "set xs \<subseteq> set keep"
+  assumes disj: "set f_args \<inter>\<^sub>\<emptyset> set xs" "set bs \<inter>\<^sub>\<emptyset> set xs"
+  assumes trace: "\<And>i. i < length ts \<Longrightarrow> frgt \<turnstile> (ts ! i, vs_b, vs_arg) \<Rightarrow>\<^bsup>hTs ! i\<^esup>  Value (vs ! i)"
+  assumes sem: "\<And>i s.
+    \<lbrakk> i < length ts; relate_exec_state f_args bs vs_arg vs_b s \<rbrakk> \<Longrightarrow>
+    \<exists>k cT s'. (to_imp_tc f_args crgt bs (xs ! i) keep (ts ! i), s) \<Rightarrow>\<^bsup>(k, cT)\<^esup>  (s', False) \<and>
+              rel_trace_to_leaf crgt f_args (xs ! i) (hTs ! i) (Value (vs ! i)) cT s' False \<and>
+              s' (xs ! i) = (vs ! i) \<and> s' = s on set f_args \<union> set bs \<union> set keep - {xs ! i}"
+  obtains k cT s' where
+    "(mk_seqs (generate (\<lambda>i. to_imp_tc f_args crgt bs (xs ! i) keep (ts ! i)) (length ts)), s) \<Rightarrow>\<^bsup>(k, cT)\<^esup> (s', False)"
+    "rel_trace_calls crgt (concat hTs) cT"
+    "lookups xs s' = vs \<and> s' = s on set f_args \<union> set bs \<union> set keep - set xs"
+  using compiled_arguments_trace[OF assms] by blast
+
+lemma copy_list_trace':
+  assumes "length xs = n"
+  assumes "length ys = n"
+  assumes "distinct ys"
+  assumes "set xs \<inter>\<^sub>\<emptyset> set ys"
+  obtains s' where
+    "(mk_seqs (generate (\<lambda>i. (ys ! i) ::= A (V (xs ! i))) (length xs)),s) \<Rightarrow>\<^bsup>(Suc (2 * length xs), [])\<^esup> (s', False)"
+    "lookups ys s' = lookups xs s" "s' = s on (- set ys)"
+  using copy_list_trace[where xs = xs and ys = ys] assms by auto
+
 
 theorem compiler_rel_trace:
-  fixes hT :: HOL_TCN_Timing.trace
   assumes "invar t"
-  assumes "frgt \<turnstile> (t,vs_b,vs_arg) \<Rightarrow>\<^bsup>hT \<^esup> hl"
-  assumes "compiler_args_invar crgt f_args bs keep t"
+  assumes "frgt \<turnstile> (t,vs_b,vs_arg) \<Rightarrow>\<^bsup> hT :: HOL_TCN_Timing.trace \<^esup> hl"
+  assumes "compiler_invar crgt f_args bs keep t"
   assumes "relate_rgt_correctness frgt crgt (calls_r t)"
   assumes "relate_exec_state f_args bs vs_arg vs_b s"
-  shows "\<exists>k cT cl s'.
-    (to_imp_tc f_args crgt bs r keep t,s)\<Rightarrow>\<^bsup>(k, cT)\<^esup> (s',cl)
+  shows "\<exists>k cT s' cl.
+    (to_imp_tc f_args crgt bs r keep t,s)\<Rightarrow>\<^bsup>(k, cT)\<^esup> (s', cl)
     \<and> rel_trace_to_leaf crgt f_args r hT hl cT s' cl"
 using assms(2) assms(1,3-) proof (induction arbitrary: bs keep s r crgt rule: htrace_to_leaf_induct)
   case (hLet frgt t1 vs_b vs_arg T1 v1 t2 T2 l2 T)
@@ -658,65 +1015,56 @@ using assms(2) assms(1,3-) proof (induction arbitrary: bs keep s r crgt rule: ht
   let ?c1 = "to_imp_tc f_args crgt bs ?r1 keep t1"
   let ?c2 = "to_imp_tc f_args crgt (?r1 # bs) r (?r1 # keep) t2"
 
-  (* assumptions and IH for t1 (and some stuff for t2) *)
+  (* solve assumptions, and obtain IH for t1 *)
 
-  have no_tails1: "\<not> HOL_TCN_Timing.tails t1" using hLet by simp
-  have invar: "HOL_TCN_Timing.invar t1" "HOL_TCN_Timing.invar t2" using hLet by simp_all
+  from hLet.prems have
+      no_tails1: "\<not> HOL_TCN_Timing.tails t1"
+      and invar: "HOL_TCN_Timing.invar t1" "HOL_TCN_Timing.invar t2"
+    by simp_all
 
-  have args_invar1: "compiler_args_invar crgt f_args bs keep t1"
-    using hLet.prems compiler_args_invar_subset[where t' = "LET t1 IN t2"] by simp
+  from hLet.prems compiler_invar_let
+  have comp_invar:
+      "compiler_invar crgt f_args bs keep t1"
+      "compiler_invar crgt f_args (?r1 # bs) (?r1 # keep) t2" by auto
 
-  have rel_rgt: "relate_rgt_correctness frgt crgt (calls_r t1)" "relate_rgt_correctness frgt crgt (calls_r t2)"
-    using hLet unfolding relate_rgt_correctness_def by simp_all
+  from hLet.prems
+  have rel_rgt:
+      "relate_rgt_correctness frgt crgt (calls_r t1)"
+      "relate_rgt_correctness frgt crgt (calls_r t2)"
+    unfolding relate_rgt_correctness_def by simp_all
 
-  have rel_state1: "relate_exec_state f_args bs vs_arg vs_b s" using hLet by blast
+  from hLet.prems have rel_state1: "relate_exec_state f_args bs vs_arg vs_b s" by blast
 
-  from hLet.hyps obtain f z1 where "(f,frgt) \<turnstile> (t1,vs_b,vs_arg) \<Rightarrow>\<^bsup>z1\<^esup> v1"
-    using trace_val_to_semantics by blast
-  then obtain f_c z1_c s2 where corr1:
-      "f_c \<turnstile> (?c1,s) \<Rightarrow>\<^bsup>z1_c\<^esup> s2" "s2 ?r1 = v1"
-      "s2 = s on set f_args \<union> set bs \<union> set keep - {?r1}"
-    using compiler_correct_no_tails[where t = t1] no_tails1 args_invar1 rel_rgt(1) rel_state1 by blast
+  from
+    hLet.IH(1)[OF invar(1) comp_invar(1) rel_rgt(1) rel_state1] rel_trace_to_leaf_cl  (* why does this need to be instantiated??? clean up *)
+    compiler_augment_rel_trace[where t = t1, OF no_tails1 hLet.hyps(1) comp_invar(1) rel_rgt(1) rel_state1]
+  obtain k1 cT1 s2 where
+      ih1:
+        "(to_imp_tc f_args crgt bs ?r1 keep t1, s) \<Rightarrow>\<^bsup>(k1, cT1)\<^esup>  (s2, False)"
+        "rel_trace_to_leaf crgt f_args ?r1 T1 (Value v1) cT1 s2 False"
+      and corr1: "s2 ?r1 = v1" "s2 = s on set f_args \<union> set bs \<union> set keep - {?r1}"
+    by (metis (full_types))
 
-  obtain k1 cT1 s2' cl1 where ih1:
-      "(?c1,s)\<Rightarrow>\<^bsup>(k1,cT1)\<^esup> (s2',cl1)" "rel_trace_to_leaf crgt f_args ?r1 T1 (Value v1) cT1 s2' cl1"
-    using hLet.IH(1) invar(1) args_invar1 rel_rgt(1) rel_state1 by blast
-  then have [simp]: "\<not> cl1" unfolding rel_trace_to_leaf_def by simp
+  (* solve assumptions and obtain IH for t2 *)
 
-  have [simp]: "s2' = s2"
-    using corr1(1) trace_nontail_has_bigstep[OF ih1(1) \<open>\<not> cl1\<close>] determ(2) by blast
-
-  (* assumptions and IH for t2 *)
-
-  have "?r1 \<notin> set f_args"
-    apply (rule contra_subsetD[OF _ fresh_not_in_stale])
-    unfolding stale_registers_def by simp
-  moreover have "?r1 \<notin> set (call_registers crgt t2)"
-    apply (rule contra_subsetD[OF _ fresh_not_in_stale])
-    using call_registers_set unfolding stale_registers_def by auto
-  moreover have "compiler_args_invar crgt f_args bs keep t2"
-    using hLet.prems compiler_args_invar_subset[where t' = "LET t1 IN t2"] by simp
-  ultimately have args_invar2: "compiler_args_invar crgt f_args (?r1 # bs) (?r1 # keep) t2"
-    using hLet.prems(3) unfolding compiler_args_invar_def by auto
-
-  have s_like_s2: "s2 = s on set f_args \<union> set bs \<union> set keep" (* TODO *)
-    by (smt (verit) DiffI Un_iff eq_on_def fresh_not_in_stale corr1(3) set_append singletonD stale_registers_def)
+  have "s2 = s on set f_args \<union> set bs \<union> set keep" (* TODO *)
+    by (smt (verit) DiffI Un_iff eq_on_def fresh_not_in_stale corr1(2) set_append singletonD stale_registers_def)
   then have rel_state2: "relate_exec_state f_args (?r1 # bs) vs_arg (v1 # vs_b) s2"
-    using hLet.prems(4) unfolding relate_exec_state_def using corr1 by fastforce
+    using hLet.prems(4) unfolding relate_exec_state_def using corr1(1) by fastforce
 
   obtain k2 cT2 s3' cl2 where ih2:
       "(?c2,s2)\<Rightarrow>\<^bsup>(k2,cT2)\<^esup> (s3',cl2)" "rel_trace_to_leaf crgt f_args r T2 l2 cT2 s3' cl2"
-    using hLet.IH(2) invar(2) args_invar2 rel_rgt(2) rel_state2 by blast
+    using hLet.IH(2) invar(2) comp_invar(2) rel_rgt(2) rel_state2 by blast
 
   (* putting it together *)
 
   show ?case unfolding to_imp_tc.simps Let_def
   proof (repeat \<open>rule exI\<close>; repeat \<open>rule conjI\<close>)
     show "(?c1;; ?c2,s) \<Rightarrow>\<^bsup>(k1 + k2, cT1 @ cT2)\<^esup> (s3', cl2)"
-      using ttrace_to_leaf.tSeq ih1(1)[simplified \<open>\<not> cl1\<close> \<open>s2' = s2\<close>] ih2(1) by blast
+      using ttrace_to_leaf.tSeq ih1(1) ih2(1) by blast
   next
     show "rel_trace_to_leaf crgt f_args r T l2 (cT1 @ cT2) s3' cl2"
-      using hLet.hyps(3) rel_trace_append ih1(2) ih2(2)
+      using hLet.hyps(3) rel_trace_to_leaf_append ih1(2) ih2(2)
       unfolding rel_trace_to_leaf_def by blast
   qed
 next
@@ -753,17 +1101,359 @@ next
       unfolding rel_trace_to_leaf_def rel_trace_calls_def rel_trace_call_def by simp
   qed
 next
-  case (hIfTrue frgt t1 bs xs T1 v1 t2 T2 l2 T t3)
-  then show ?case sorry
+  case (hIfTrue frgt t1 vs_b vs_arg T1 v1 t2 T2 l2 T t3)
+
+  let ?r1 = "fresh' (stale_registers f_args crgt bs keep (IF t1\<noteq>0 THEN t2 ELSE t3)) ''If.x''"
+  let ?c1 = "to_imp_tc f_args crgt bs ?r1 keep t1"
+  let ?c2 = "to_imp_tc f_args crgt bs r keep t2"
+  let ?c3 = "to_imp_tc f_args crgt bs r keep t3"
+
+  from hIfTrue.prems
+  have no_tails: "\<not> HOL_TCN_Timing.tails t1"
+      and invar: "HOL_TCN_Timing.invar t1" "HOL_TCN_Timing.invar t2" by simp_all
+
+  from compiler_invar_if[OF hIfTrue.prems(2)]
+  have comp_invar:
+      "compiler_invar crgt f_args bs keep t1"
+      "compiler_invar crgt f_args bs keep t2" by auto
+
+  from hIfTrue.prems
+  have rel_rgt:
+      "relate_rgt_correctness frgt crgt (calls_r t1)"
+      "relate_rgt_correctness frgt crgt (calls_r t2)"
+    unfolding relate_rgt_correctness_def by simp_all
+
+  from hIfTrue.prems have rel_state1: "relate_exec_state f_args bs vs_arg vs_b s" by blast
+
+  (* t1 *)
+
+  from
+    hIfTrue.IH(1)[OF invar(1) comp_invar(1) rel_rgt(1) rel_state1] rel_trace_to_leaf_cl  (* why does this need to be instantiated??? clean up *)
+    compiler_augment_rel_trace[where t = t1, OF no_tails hIfTrue.hyps(1) comp_invar(1) rel_rgt(1) rel_state1]
+  obtain k1 cT1 s2 where
+      ih1:
+        "(to_imp_tc f_args crgt bs ?r1 keep t1, s) \<Rightarrow>\<^bsup>(k1, cT1)\<^esup>  (s2, False)"
+        "rel_trace_to_leaf crgt f_args ?r1 T1 (Value v1) cT1 s2 False"
+      and corr1: "s2 ?r1 = v1" "s2 = s on set f_args \<union> set bs \<union> set keep - {?r1}"
+    by (metis (full_types))
+
+  (* t2 *)
+
+  have "s2 = s on set f_args \<union> set bs \<union> set keep" (* TODO *)
+    by (smt (verit) DiffI Un_iff eq_on_def fresh_not_in_stale corr1(2) set_append singletonD stale_registers_def)
+  then have rel_state2: "relate_exec_state f_args bs vs_arg vs_b s2"
+    using hIfTrue.prems unfolding relate_exec_state_def by fastforce
+
+  from hIfTrue.IH(2) invar(2) comp_invar(2) rel_rgt(2) rel_state2
+  obtain k2 cT2 s3' cl2 where ih2:
+      "(?c2,s2)\<Rightarrow>\<^bsup>(k2,cT2)\<^esup> (s3',cl2)" "rel_trace_to_leaf crgt f_args r T2 l2 cT2 s3' cl2"
+    by blast
+
+  (* putting it together *)
+
+  show ?case unfolding to_imp_tc.simps Let_def
+  proof (repeat \<open>rule exI\<close>; repeat \<open>rule conjI\<close>)
+    show "(?c1;; IF ?r1\<noteq>0 THEN ?c2 ELSE ?c3,s) \<Rightarrow>\<^bsup>(Suc (k1 + k2), cT1 @ cT2)\<^esup> (s3', cl2)"
+    proof
+      show "(?c1,s) \<Rightarrow>\<^bsup>(k1, cT1)\<^esup> (s2, False)" using ih1(1) by simp
+      show "(IF ?r1\<noteq>0 THEN ?c2 ELSE ?c3,s2)\<Rightarrow>\<^bsup>(Suc k2, cT2)\<^esup> (s3', cl2)"
+      proof (rule ttrace_to_leaf.tIfTrue)
+        show "s2 ?r1 \<noteq> 0" using hIfTrue.hyps corr1(1) by simp
+        show "(?c2, s2) \<Rightarrow>\<^bsup>(k2, cT2)\<^esup>  (s3', cl2)" using ih2(1) by blast
+      qed simp
+    qed simp_all
+    show "rel_trace_to_leaf crgt f_args r T l2 (cT1 @ cT2) s3' cl2"
+      using hIfTrue.hyps(4) rel_trace_to_leaf_append ih1(2) ih2(2)
+      unfolding rel_trace_to_leaf_def by blast
+  qed
 next
-  case (hIfFalse frgt t1 bs xs T1 v1 t3 T3 l3 T t2)
-  then show ?case sorry
+  case (hIfFalse frgt t1 vs_b vs_arg T1 v1 t3 T3 l3 T t2)
+
+  let ?r1 = "fresh' (stale_registers f_args crgt bs keep (IF t1\<noteq>0 THEN t2 ELSE t3)) ''If.x''"
+  let ?c1 = "to_imp_tc f_args crgt bs ?r1 keep t1"
+  let ?c2 = "to_imp_tc f_args crgt bs r keep t2"
+  let ?c3 = "to_imp_tc f_args crgt bs r keep t3"
+
+  from hIfFalse.prems
+  have no_tails: "\<not> HOL_TCN_Timing.tails t1"
+      and invar: "HOL_TCN_Timing.invar t1" "HOL_TCN_Timing.invar t3" by simp_all
+
+  from compiler_invar_if[OF hIfFalse.prems(2)]
+  have comp_invar:
+      "compiler_invar crgt f_args bs keep t1"
+      "compiler_invar crgt f_args bs keep t3" by auto
+
+  from hIfFalse.prems
+  have rel_rgt:
+      "relate_rgt_correctness frgt crgt (calls_r t1)"
+      "relate_rgt_correctness frgt crgt (calls_r t3)"
+    unfolding relate_rgt_correctness_def by simp_all
+
+  from hIfFalse.prems have rel_state1: "relate_exec_state f_args bs vs_arg vs_b s" by blast
+
+  (* t1 *)
+
+  from
+    hIfFalse.IH(1)[OF invar(1) comp_invar(1) rel_rgt(1) rel_state1] rel_trace_to_leaf_cl  (* why does this need to be instantiated??? clean up *)
+    compiler_augment_rel_trace[where t = t1, OF no_tails hIfFalse.hyps(1) comp_invar(1) rel_rgt(1) rel_state1]
+  obtain k1 cT1 s2 where
+      ih1:
+        "(to_imp_tc f_args crgt bs ?r1 keep t1, s) \<Rightarrow>\<^bsup>(k1, cT1)\<^esup>  (s2, False)"
+        "rel_trace_to_leaf crgt f_args ?r1 T1 (Value v1) cT1 s2 False"
+      and corr1: "s2 ?r1 = v1" "s2 = s on set f_args \<union> set bs \<union> set keep - {?r1}"
+    by (metis (full_types))
+
+  (* t2 *)
+
+  have "s2 = s on set f_args \<union> set bs \<union> set keep" (* TODO *)
+    by (smt (verit) DiffI Un_iff eq_on_def fresh_not_in_stale corr1(2) set_append singletonD stale_registers_def)
+  then have rel_state2: "relate_exec_state f_args bs vs_arg vs_b s2"
+    using hIfFalse.prems unfolding relate_exec_state_def by fastforce
+
+  from hIfFalse.IH(2) invar(2) comp_invar(2) rel_rgt(2) rel_state2
+  obtain k2 cT2 s3' cl2 where ih2:
+      "(?c3,s2)\<Rightarrow>\<^bsup>(k2,cT2)\<^esup> (s3',cl2)" "rel_trace_to_leaf crgt f_args r T3 l3 cT2 s3' cl2"
+    by blast
+
+  (* putting it together *)
+
+  show ?case unfolding to_imp_tc.simps Let_def
+  proof (repeat \<open>rule exI\<close>; repeat \<open>rule conjI\<close>)
+    show "(?c1;; IF ?r1\<noteq>0 THEN ?c2 ELSE ?c3,s) \<Rightarrow>\<^bsup>(Suc (k1 + k2), cT1 @ cT2)\<^esup> (s3', cl2)"
+    proof
+      show "(?c1,s) \<Rightarrow>\<^bsup>(k1, cT1)\<^esup> (s2, False)" using ih1(1) by simp
+      show "(IF ?r1\<noteq>0 THEN ?c2 ELSE ?c3,s2)\<Rightarrow>\<^bsup>(Suc k2, cT2)\<^esup> (s3', cl2)"
+      proof (rule ttrace_to_leaf.tIfFalse)
+        show "s2 ?r1 = 0" using hIfFalse.hyps corr1(1) by simp
+        show "(?c3, s2) \<Rightarrow>\<^bsup>(k2, cT2)\<^esup>  (s3', cl2)" using ih2(1) by blast
+      qed simp
+    qed simp_all
+    show "rel_trace_to_leaf crgt f_args r T l3 (cT1 @ cT2) s3' cl2"
+      using hIfFalse.hyps(4) rel_trace_to_leaf_append ih1(2) ih2(2)
+      unfolding rel_trace_to_leaf_def by blast
+  qed
 next
-  case (hCall g T_g frgt gr vs ts Ts bs xs T v)
-  then show ?case sorry
+  case (hCall g T_g frgt gr vs ts hTs vs_b vs_arg T v)
+
+  let ?g = "f_from_frgt frgt gr"
+  let ?T_g = "T_f_from_frgt frgt gr"
+
+  let ?xs = "make_n_fresh (stale_registers f_args crgt bs keep (hCall gr ts)) ''Call.x.'' (length ts)"
+  let ?c_arg = "\<lambda>i. to_imp_tc f_args crgt bs (?xs ! i) (?xs @ keep) (ts ! i)"
+  let ?c1 = "mk_seqs (generate ?c_arg (length ts))"
+
+  (* part 1: computing the arguments *)
+
+  from hCall.prems
+  have no_tails: "\<not> HOL_TCN_Timing.tails (ts ! i)" and invar: "HOL_TCN_Timing.invar (ts ! i)"
+    if "i < length ts" for i using that by simp_all
+
+  from compiler_invar_call[OF hCall.prems(2)]
+  have comp_invar: "compiler_invar crgt f_args bs (?xs @ keep) (ts ! i)"
+    if "i < length ts" for i using that by simp
+
+  have "calls_r (ts ! i) \<subseteq> calls_r (hCall gr ts)" if "i < length ts" for i using that by fastforce
+  with hCall.prems have rel_rgt:
+      "relate_rgt_correctness frgt crgt (calls_r (ts ! i))"
+    if "i < length ts" for i using that unfolding relate_rgt_correctness_def by blast
+
+  from hCall.IH
+  have htrace: "frgt \<turnstile> (ts ! i, vs_b, vs_arg) \<Rightarrow>\<^bsup>hTs ! i\<^esup>  Value (vs ! i)"
+    if "i < length ts" for i using that by blast
+
+  have aug_ih: "\<exists>k cT s'. (?c_arg i, s) \<Rightarrow>\<^bsup>(k, cT)\<^esup>  (s', False) \<and>
+                      rel_trace_to_leaf crgt f_args (?xs ! i) (hTs ! i) (Value (vs ! i)) cT s' False \<and>
+                      s' (?xs ! i) = vs ! i \<and> s' = s on set f_args \<union> set bs \<union> set (?xs @ keep) - {?xs ! i}"
+    if "relate_exec_state f_args bs vs_arg vs_b s" "i < length ts" for i s
+  proof goal_cases case 1
+
+    from hCall.IH invar comp_invar rel_rgt that
+    obtain k cT s' where trace:
+      "(?c_arg i, s) \<Rightarrow>\<^bsup>(k, cT)\<^esup>  (s', False)"
+      "rel_trace_to_leaf crgt f_args (?xs ! i) (hTs ! i) (Value (vs ! i)) cT s' False"
+      using rel_trace_to_leaf_cl by (metis (full_types))
+
+    moreover with compiler_augment_rel_trace no_tails htrace comp_invar rel_rgt that
+    have "s' (?xs ! i) = vs ! i \<and> s' = s on set f_args \<union> set bs \<union> set (?xs @ keep) - {?xs ! i}"
+      by metis
+
+    ultimately show ?case by blast
+  qed
+
+  have lengths: "length vs = length ts" "length ?xs = length ts" "length hTs = length ts"
+    using hCall.hyps unfolding make_n_fresh_def generate_def by simp_all
+  have *: "distinct ?xs" using distinct_make_n_fresh by blast
+  have **: "set ?xs \<subseteq> set (?xs @ keep)" by simp
+  have ***: "set f_args \<inter>\<^sub>\<emptyset> set ?xs" "set bs \<inter>\<^sub>\<emptyset> set ?xs"
+    unfolding stale_registers_def using make_n_fresh_not_in_stale by fastforce+
+
+  from compiled_arguments_trace[OF lengths hCall.prems(4) * ** *** htrace aug_ih] (* TODO *)
+  obtain k1 cTs s2 where
+      trace1: "(?c1,s) \<Rightarrow>\<^bsup>(k1, cTs)\<^esup> (s2, False)" "rel_trace_calls crgt (concat hTs) cTs"
+      and corr1: "lookups ?xs s2 = vs" "s2 = s on set f_args \<union> set bs \<union> set (?xs @ keep) - set ?xs"
+    by blast
+
+  (* part 2: copying from temporaries to argument registers *)
+
+  let ?c2 = "mk_seqs (generate (\<lambda>i. (args_from_crgt crgt gr ! i) ::= A (V (?xs ! i))) (length ts))"
+  let ?k2 = "Suc (2 * length ts)"
+
+  have "set (args_from_crgt crgt gr) \<subseteq> set (stale_registers f_args crgt bs keep (hCall gr ts))"
+    unfolding stale_registers_def call_registers_def using calls'_set by auto
+  then have 1: "set ?xs \<inter>\<^sub>\<emptyset> set (args_from_crgt crgt gr)"
+    using make_n_fresh_not_in_stale by blast
+  moreover have 2: "distinct (args_from_crgt crgt gr)"
+    using hCall.prems unfolding compiler_invar_def calls'_set by simp
+  moreover have 3: "length ?xs = length ts"
+    unfolding make_n_fresh_def generate_def by simp
+  moreover have 4: "length (args_from_crgt crgt gr) = length ts"
+    using hCall.prems unfolding compiler_invar_def calls_n_set by simp
+
+  ultimately obtain s3 where trace2: "(?c2, s2) \<Rightarrow>\<^bsup>(?k2, [])\<^esup> (s3,False)"
+       "lookup_args crgt gr s3 = lookups ?xs s2" "s3 = s2 on - set (args_from_crgt crgt gr)"
+    using copy_list_trace'[OF 3 4 2 1] by auto (* ? *)
+
+  (* part 3: calling g *)
+
+  let ?gcom = "com_from_crgt crgt gr" and ?gret = "ret_from_crgt crgt gr" and ?gv = "f_from_frgt frgt gr (lookup_args crgt gr s3)"
+  let ?c3 = "CALL ?gcom RETURN ?gret :: tcom"
+  let ?k3 = "0 :: nat"
+  let ?s4 = "s3(?gret := ?gv)"
+
+  have "terminates_with_res_IMP ?gcom s3 ?gret ?gv" using hCall.prems unfolding relate_rgt_correctness_def by simp
+  then obtain z3 s4' where "(?gcom, s3) \<Rightarrow>\<^bsup>z3\<^esup> s4'" "s4' ?gret = ?gv"
+    unfolding terminates_with_res_IMP_def terminates_with_res_pred_time_IMP_def terminates_with_pred_time_IMP_def by blast
+  then have trace3: "(?c3, s3) \<Rightarrow>\<^bsup>(?k3, [(?gcom, s3)])\<^esup> (?s4, False)" using ttrace_to_leaf.tCall by metis
+
+  have g_args: "lookup_args crgt gr s3 = vs" using trace2 corr1 by simp
+  then have g_call: "?gv = v" using trace1 hCall split_from_frgt by auto
+
+  (* part 4: copying to r *)
+
+  let ?c4 = "r ::= A (V (ret_from_crgt crgt gr)) :: tcom"
+
+  let ?k4 = "Suc (Suc 0)"
+  let ?s5 = "?s4(r := aval (A (V ?gret)) ?s4)"
+  have trace4: "(?c4, ?s4) \<Rightarrow>\<^bsup>(?k4, [])\<^esup> (?s5, False)" using ttrace_to_leaf.tAssign by blast
+  then have s5: "?s5 = ?s4(r := v)" using g_call trace3 by simp
+
+  (* putting it together *)
+
+  show ?case unfolding to_imp_tc.simps Let_def split_beta
+  proof (repeat \<open>rule exI\<close>; repeat \<open>rule conjI\<close>)
+    show "(?c1;; ?c2;; ?c3;; ?c4, s) \<Rightarrow>\<^bsup>(k1 + ?k2 + ?k3 + ?k4, cTs @ [(?gcom, s3)])\<^esup> (?s5,False)"
+      apply (repeat \<open>rule ttrace_to_leaf.tSeq\<close>)
+      using trace1 trace2 trace3 trace4 by blast+ auto
+  next
+    have "rel_trace_call crgt gr vs ?gcom s3"
+      unfolding rel_trace_call_def using g_args by blast
+    then have *: "rel_trace_calls crgt [(gr, vs)] [(?gcom, s3)]"
+      unfolding rel_trace_calls_def by simp
+
+    have **: "rel_leaf_state crgt f_args r (Value v) ?s5 False"
+      using g_call by simp
+    
+    from * ** trace1(2)
+    show "rel_trace_to_leaf crgt f_args r T (Value v) (cTs @ [(?gcom, s3)]) ?s5 False"
+      unfolding rel_trace_to_leaf_def \<open>T = concat hTs @ [(gr, vs)]\<close>
+      using rel_trace_calls_append by blast
+  qed
 next
-  case (hTail vs ts Ts frgt bs xs T)
-  then show ?case sorry
+  case (hTail vs ts hTs frgt vs_b vs_arg T)
+
+  let ?xs = "make_n_fresh (stale_registers f_args crgt bs keep (hTAIL ts)) ''TAIL.x.'' (length ts)"
+  let ?c_arg = "\<lambda>i. to_imp_tc f_args crgt bs (?xs ! i) (?xs @ keep) (ts ! i)"
+  let ?c1 = "mk_seqs (generate ?c_arg (length ts))"
+
+  (* part 1: computing the arguments *)
+
+  from hTail.prems
+  have no_tails: "\<not> HOL_TCN_Timing.tails (ts ! i)" and invar: "HOL_TCN_Timing.invar (ts ! i)"
+    if "i < length ts" for i using that by simp_all
+
+  from compiler_invar_tail[OF hTail.prems(2)]
+  have comp_invar: "compiler_invar crgt f_args bs (?xs @ keep) (ts ! i)"
+    if "i < length ts" for i using that by simp
+
+  have "calls_r (ts ! i) \<subseteq> calls_r (hTAIL ts)" if "i < length ts" for i using that by fastforce
+  with hTail.prems have rel_rgt:
+      "relate_rgt_correctness frgt crgt (calls_r (ts ! i))"
+    if "i < length ts" for i using that unfolding relate_rgt_correctness_def by blast
+
+  from hTail.IH
+  have htrace: "frgt \<turnstile> (ts ! i, vs_b, vs_arg) \<Rightarrow>\<^bsup>hTs ! i\<^esup>  Value (vs ! i)"
+    if "i < length ts" for i using that by blast
+
+  have aug_ih: "\<exists>k cT s'. (?c_arg i, s) \<Rightarrow>\<^bsup>(k, cT)\<^esup>  (s', False) \<and>
+                      rel_trace_to_leaf crgt f_args (?xs ! i) (hTs ! i) (Value (vs ! i)) cT s' False \<and>
+                      s' (?xs ! i) = vs ! i \<and> s' = s on set f_args \<union> set bs \<union> set (?xs @ keep) - {?xs ! i}"
+    if "relate_exec_state f_args bs vs_arg vs_b s" "i < length ts" for i s
+  proof goal_cases case 1
+
+    from hTail.IH invar comp_invar rel_rgt that
+    obtain k cT s' where trace:
+      "(?c_arg i, s) \<Rightarrow>\<^bsup>(k, cT)\<^esup>  (s', False)"
+      "rel_trace_to_leaf crgt f_args (?xs ! i) (hTs ! i) (Value (vs ! i)) cT s' False"
+      using rel_trace_to_leaf_cl by (metis (full_types))
+
+    moreover with compiler_augment_rel_trace no_tails htrace comp_invar rel_rgt that
+    have "s' (?xs ! i) = vs ! i \<and> s' = s on set f_args \<union> set bs \<union> set (?xs @ keep) - {?xs ! i}"
+      by metis
+
+    ultimately show ?case by blast
+  qed
+
+  have lengths: "length vs = length ts" "length ?xs = length ts" "length hTs = length ts"
+    using hTail.hyps unfolding make_n_fresh_def generate_def by simp_all
+  have *: "distinct ?xs" using distinct_make_n_fresh by blast
+  have **: "set ?xs \<subseteq> set (?xs @ keep)" by simp
+  have ***: "set f_args \<inter>\<^sub>\<emptyset> set ?xs" "set bs \<inter>\<^sub>\<emptyset> set ?xs"
+    unfolding stale_registers_def using make_n_fresh_not_in_stale by fastforce+
+
+  from compiled_arguments_trace[OF lengths hTail.prems(4) * ** *** htrace aug_ih] (* TODO *)
+  obtain k1 cTs s2 where
+      trace1: "(?c1,s) \<Rightarrow>\<^bsup>(k1, cTs)\<^esup> (s2, False)" "rel_trace_calls crgt (concat hTs) cTs"
+      and corr1: "lookups ?xs s2 = vs" "s2 = s on set f_args \<union> set bs \<union> set (?xs @ keep) - set ?xs"
+    by blast
+
+  (* part 2: copying from temporaries to argument registers *)
+
+  let ?c2 = "mk_seqs (generate (\<lambda>i. (f_args ! i) ::= A (V (?xs ! i))) (length ts))"
+  let ?k2 = "Suc (2 * length ts)"
+
+  have "set f_args \<subseteq> set (stale_registers f_args crgt bs keep (hTAIL ts))"
+    unfolding stale_registers_def call_registers_def using calls'_set by auto
+  then have 1: "set ?xs \<inter>\<^sub>\<emptyset> set f_args"
+    using make_n_fresh_not_in_stale by blast
+  moreover have 2: "distinct f_args"
+    using hTail.prems unfolding compiler_invar_def calls'_set by simp
+  moreover have 3: "length ?xs = length ts"
+    unfolding make_n_fresh_def generate_def by simp
+  moreover have 4: "length f_args = length ts"
+    using hTail.prems unfolding compiler_invar_def calls_n_set sorry (* need to change invariant *)
+
+  ultimately obtain s3 where trace2: "(?c2, s2) \<Rightarrow>\<^bsup>(?k2, [])\<^esup> (s3,False)"
+       "lookups f_args s3 = lookups ?xs s2" "s3 = s2 on - set f_args"
+    using copy_list_trace'[OF 3 4 2 1] by auto (* ? *)
+
+  have g_args: "lookups f_args s3 = vs" using trace2 corr1 by simp
+
+  (* putting it together *)
+
+  show ?case unfolding to_imp_tc.simps Let_def split_beta
+  proof (repeat \<open>rule exI\<close>; repeat \<open>rule conjI\<close>)
+    show "(?c1;; ?c2;; tTAIL, s) \<Rightarrow>\<^bsup>(k1 + ?k2 + 5, cTs)\<^esup> (s3, True)"
+      apply (repeat \<open>rule ttrace_to_leaf.tSeq ttrace_to_leaf.tTail\<close>)
+      using trace1 trace2 by blast+ simp
+  next
+    have **: "rel_leaf_state crgt f_args r (Tail vs) s3 True"
+      using g_args by simp
+
+    from * ** trace1(2)
+    show "rel_trace_to_leaf crgt f_args r T (Tail vs) cTs s3 True"
+      unfolding rel_trace_to_leaf_def \<open>T = concat hTs\<close>
+      using rel_trace_calls_append by blast
+  qed
 qed
 
 (* lemma "\<exists>c. \<forall>s. tstruct_k t_imp + something \<le> c * interp_time frgt (time_to_tail frgt vs_b vs_arg t)" oops *)
